@prefix : <https://purls.helmholtz-metadaten.de/ptro#> .
@prefix owl: <http://www.w3.org/2002/07/owl#> .
@prefix rdf: <http://www.w3.org/1999/02/22-rdf-syntax-ns#> .
@prefix xml: <http://www.w3.org/XML/1998/namespace> .
@prefix xsd: <http://www.w3.org/2001/XMLSchema#> .
@prefix rdfs: <http://www.w3.org/2000/01/rdf-schema#> .
@base <https://purls.helmholtz-metadaten.de/ptro#> .

<https://purls.helmholtz-metadaten.de/ptro> rdf:type owl:Ontology ;
                                             owl:versionIRI <https://purls.helmholtz-metadaten.de/ptro/2025-11-25> ;
                                             <http://purl.org/dc/elements/1.1/creator> "DKFZ-E220" ;
                                             <http://purl.org/dc/terms/license> "https://creativecommons.org/licenses/by/4.0/" ;
                                             rdfs:comment "The Ontology for Preclinical Trials in Radiation Oncology (PTRO), is a domain-specific ontology designed to integrate SEND-standardized preclinical data using semantic web technologies. PTRO incorporates the Semantic Types Ontology (STY) as a framework for broad concept categorization." ;
                                             owl:versionInfo "0.1 alpha" .

#################################################################
#    Annotation properties
#################################################################

###  http://data.bioontology.org/metadata/prefixIRI
<http://data.bioontology.org/metadata/prefixIRI> rdf:type owl:AnnotationProperty .


###  http://purl.org/dc/elements/1.1/creator
<http://purl.org/dc/elements/1.1/creator> rdf:type owl:AnnotationProperty .


###  http://purl.org/dc/terms/license
<http://purl.org/dc/terms/license> rdf:type owl:AnnotationProperty .


###  http://www.w3.org/2004/02/skos/core#altLabel
<http://www.w3.org/2004/02/skos/core#altLabel> rdf:type owl:AnnotationProperty ;
                                               rdfs:subPropertyOf rdfs:label .


###  http://www.w3.org/2004/02/skos/core#definition
<http://www.w3.org/2004/02/skos/core#definition> rdf:type owl:AnnotationProperty ;
                                                 rdfs:subPropertyOf <http://www.w3.org/2004/02/skos/core#note> .


###  http://www.w3.org/2004/02/skos/core#exactMatch
<http://www.w3.org/2004/02/skos/core#exactMatch> rdf:type owl:AnnotationProperty .


###  http://www.w3.org/2004/02/skos/core#notation
<http://www.w3.org/2004/02/skos/core#notation> rdf:type owl:AnnotationProperty .


###  http://www.w3.org/2004/02/skos/core#note
<http://www.w3.org/2004/02/skos/core#note> rdf:type owl:AnnotationProperty .


#################################################################
#    Datatypes
#################################################################

###  http://www.w3.org/2001/XMLSchema#gYear
xsd:gYear rdf:type rdfs:Datatype .


#################################################################
#    Object Properties
#################################################################

###  http://www.cancerdata.org/roo/P100040
<http://www.cancerdata.org/roo/P100040> rdf:type owl:ObjectProperty ;
                                        rdfs:domain <http://ncicb.nci.nih.gov/xml/owl/EVS/Thesaurus.owl#C83083> ;
                                        <http://purl.org/dc/elements/1.1/creator> "Andre Dekker" ;
                                        rdfs:label "associated_with"@en ;
                                        <http://www.w3.org/2004/02/skos/core#definition> "has a significant or salient relationship to."@en .


###  http://www.w3.org/2002/07/owl#topObjectProperty
owl:topObjectProperty rdf:type owl:ObjectProperty .


###  https://purls.helmholtz-metadaten.de/ptroDKFZ000047
<https://purls.helmholtz-metadaten.de/ptroDKFZ000047> rdf:type owl:ObjectProperty ;
                                                      <http://purl.org/dc/elements/1.1/creator> "OGiraldo" ;
                                                      rdfs:label "participates_in" ;
                                                      <http://www.w3.org/2004/02/skos/core#definition> "Relation between an activity and  an entity,  at which the entity participates in some way in the activity or process." .


###  https://purls.helmholtz-metadaten.de/ptroDKFZ000048
<https://purls.helmholtz-metadaten.de/ptroDKFZ000048> rdf:type owl:ObjectProperty ;
                                                      rdfs:label "has_participant" .


###  https://purls.helmholtz-metadaten.de/ptroDKFZ000076
<https://purls.helmholtz-metadaten.de/ptroDKFZ000076> rdf:type owl:ObjectProperty ;
                                                      owl:inverseOf <https://purls.helmholtz-metadaten.de/ptroDKFZ000078> ;
                                                      rdfs:domain <http://ncicb.nci.nih.gov/xml/owl/EVS/Thesaurus.owl#C69256> ;
                                                      rdfs:range <https://purls.helmholtz-metadaten.de/ptroDKFZ000059> ;
                                                      rdfs:label "has_lab_record_id" ;
                                                      <http://www.w3.org/2004/02/skos/core#definition> "This property links a 'Subject Unique Identifie'r  to a 'Laboratory Record Identifier'" .


###  https://purls.helmholtz-metadaten.de/ptroDKFZ000077
<https://purls.helmholtz-metadaten.de/ptroDKFZ000077> rdf:type owl:ObjectProperty ;
                                                      owl:inverseOf <https://purls.helmholtz-metadaten.de/ptroDKFZ000079> ;
                                                      rdfs:domain <http://ncicb.nci.nih.gov/xml/owl/EVS/Thesaurus.owl#C69256> ;
                                                      rdfs:range <https://purls.helmholtz-metadaten.de/ptroDKFZ000050> ;
                                                      rdfs:label "has_session_id" ;
                                                      <http://www.w3.org/2004/02/skos/core#definition> "This property links a 'Subject Unique Identifier'  to a 'Treatment Session Identifier'" .


###  https://purls.helmholtz-metadaten.de/ptroDKFZ000078
<https://purls.helmholtz-metadaten.de/ptroDKFZ000078> rdf:type owl:ObjectProperty ;
                                                      rdfs:domain <https://purls.helmholtz-metadaten.de/ptroDKFZ000059> ;
                                                      rdfs:range <http://ncicb.nci.nih.gov/xml/owl/EVS/Thesaurus.owl#C69256> ;
                                                      rdfs:label "is_lab_record_id_of" .


###  https://purls.helmholtz-metadaten.de/ptroDKFZ000079
<https://purls.helmholtz-metadaten.de/ptroDKFZ000079> rdf:type owl:ObjectProperty ;
                                                      rdfs:domain <https://purls.helmholtz-metadaten.de/ptroDKFZ000050> ;
                                                      rdfs:range <http://ncicb.nci.nih.gov/xml/owl/EVS/Thesaurus.owl#C69256> ;
                                                      rdfs:label "is_session_id_of" .


###  https://purls.helmholtz-metadaten.de/ptroDKFZ000081
<https://purls.helmholtz-metadaten.de/ptroDKFZ000081> rdf:type owl:ObjectProperty ;
                                                      owl:inverseOf <https://purls.helmholtz-metadaten.de/ptroDKFZ000082> ;
                                                      rdfs:domain <http://ncicb.nci.nih.gov/xml/owl/EVS/Thesaurus.owl#C69256> ;
                                                      rdfs:range <https://purls.helmholtz-metadaten.de/ptroDKFZ000080> ;
                                                      rdfs:label "has_body_weight_id" ;
                                                      <http://www.w3.org/2004/02/skos/core#definition> "This property links a 'Subject Unique Identifie'r  to a 'Body Weigh Identifier'" .


###  https://purls.helmholtz-metadaten.de/ptroDKFZ000082
<https://purls.helmholtz-metadaten.de/ptroDKFZ000082> rdf:type owl:ObjectProperty ;
                                                      rdfs:domain <https://purls.helmholtz-metadaten.de/ptroDKFZ000080> ;
                                                      rdfs:range <http://ncicb.nci.nih.gov/xml/owl/EVS/Thesaurus.owl#C69256> ;
                                                      rdfs:label "is_body_weight_id_of" .


###  https://purls.helmholtz-metadaten.de/ptroDKFZ000086
<https://purls.helmholtz-metadaten.de/ptroDKFZ000086> rdf:type owl:ObjectProperty ;
                                                      owl:inverseOf <https://purls.helmholtz-metadaten.de/ptroDKFZ000088> ;
                                                      rdfs:domain <http://ncicb.nci.nih.gov/xml/owl/EVS/Thesaurus.owl#C69256> ;
                                                      rdfs:range <https://purls.helmholtz-metadaten.de/ptroDKFZ000087> ;
                                                      rdfs:label "has_procedure_id" ;
                                                      <http://www.w3.org/2004/02/skos/core#definition> "This property links a 'Subject Unique Identifier'  to a 'Procedure Identifier'" .


###  https://purls.helmholtz-metadaten.de/ptroDKFZ000088
<https://purls.helmholtz-metadaten.de/ptroDKFZ000088> rdf:type owl:ObjectProperty ;
                                                      rdfs:domain <https://purls.helmholtz-metadaten.de/ptroDKFZ000087> ;
                                                      rdfs:range <http://ncicb.nci.nih.gov/xml/owl/EVS/Thesaurus.owl#C69256> ;
                                                      rdfs:label "is_procedure_id_of" .


#################################################################
#    Data properties
#################################################################

###  https://purls.helmholtz-metadaten.de/ptroDKFZ000008
<https://purls.helmholtz-metadaten.de/ptroDKFZ000008> rdf:type owl:DatatypeProperty ;
                                                      rdfs:domain <http://ncicb.nci.nih.gov/xml/owl/EVS/Thesaurus.owl#C69256> ;
                                                      rdfs:range xsd:string ;
                                                      <http://purl.org/dc/elements/1.1/creator> "OGiraldo" ;
                                                      rdfs:isDefinedBy "https://library.cdisc.org/browser" ;
                                                      rdfs:label "Study_Identifier" ;
                                                      <http://www.w3.org/2004/02/skos/core#altLabel> "STUDYID" ;
                                                      <http://www.w3.org/2004/02/skos/core#definition> "Unique identifier for a study." ;
                                                      <http://www.w3.org/2004/02/skos/core#exactMatch> "Thesaurus:C83082 (http://ncicb.nci.nih.gov/xml/owl/EVS/Thesaurus.owl#C83082)" .


###  https://purls.helmholtz-metadaten.de/ptroDKFZ000009
<https://purls.helmholtz-metadaten.de/ptroDKFZ000009> rdf:type owl:DatatypeProperty ;
                                                      rdfs:domain <http://ncicb.nci.nih.gov/xml/owl/EVS/Thesaurus.owl#C14238> ;
                                                      rdfs:range xsd:string ;
                                                      <http://purl.org/dc/elements/1.1/creator> "OGiraldo" ;
                                                      rdfs:comment "a.k.a 'Subject Id' at RPB." ;
                                                      rdfs:isDefinedBy "https://library.cdisc.org/browser" ;
                                                      rdfs:label "Unique_Subject_Identifier" ;
                                                      <http://www.w3.org/2004/02/skos/core#altLabel> "USUBJID" ;
                                                      <http://www.w3.org/2004/02/skos/core#definition> "Identifier used to uniquely identify a subject across all studies for all applications or submissions involving the product." .


###  https://purls.helmholtz-metadaten.de/ptroDKFZ000010
<https://purls.helmholtz-metadaten.de/ptroDKFZ000010> rdf:type owl:DatatypeProperty ;
                                                      rdfs:domain <http://ncicb.nci.nih.gov/xml/owl/EVS/Thesaurus.owl#C14238> ;
                                                      rdfs:range xsd:string ;
                                                      <http://purl.org/dc/elements/1.1/creator> "OGiraldo" ;
                                                      rdfs:comment "a.k.a 'subject identification' at RPB." ;
                                                      rdfs:isDefinedBy "https://library.cdisc.org/browser" ;
                                                      rdfs:label "Subject_Identifier_for_the_Study" ;
                                                      <http://www.w3.org/2004/02/skos/core#altLabel> "SUBJID" ;
                                                      <http://www.w3.org/2004/02/skos/core#definition> "Subject (i.e., Animal) identifier used within the study." ;
                                                      <http://www.w3.org/2004/02/skos/core#exactMatch> "Thesaurus:C83083 (http://ncicb.nci.nih.gov/xml/owl/EVS/Thesaurus.owl#C83083)" .


###  https://purls.helmholtz-metadaten.de/ptroDKFZ000011
<https://purls.helmholtz-metadaten.de/ptroDKFZ000011> rdf:type owl:DatatypeProperty ;
                                                      rdfs:domain <http://ncicb.nci.nih.gov/xml/owl/EVS/Thesaurus.owl#C69256> ;
                                                      rdfs:range xsd:string ;
                                                      <http://purl.org/dc/elements/1.1/creator> "OGiraldo" ;
                                                      rdfs:isDefinedBy "https://library.cdisc.org/browser" ;
                                                      rdfs:label "Route_of_Administration" ;
                                                      <http://www.w3.org/2004/02/skos/core#altLabel> "EXROUTE" ;
                                                      <http://www.w3.org/2004/02/skos/core#definition> "Route of administration for EXTRT. Examples: ORAL GAVAGE, DERMAL, INTRAVENOUS." ;
                                                      <http://www.w3.org/2004/02/skos/core#exactMatch> "Thesaurus:C83121 (http://ncicb.nci.nih.gov/xml/owl/EVS/Thesaurus.owl#C83121)" .


###  https://purls.helmholtz-metadaten.de/ptroDKFZ000012
<https://purls.helmholtz-metadaten.de/ptroDKFZ000012> rdf:type owl:DatatypeProperty ;
                                                      rdfs:domain <http://ncicb.nci.nih.gov/xml/owl/EVS/Thesaurus.owl#C69256> ;
                                                      rdfs:range xsd:string ;
                                                      <http://purl.org/dc/elements/1.1/creator> "OGiraldo" ;
                                                      rdfs:isDefinedBy "https://library.cdisc.org/browser" ;
                                                      rdfs:label "Treatment_Vehicle" ;
                                                      <http://www.w3.org/2004/02/skos/core#altLabel> "EXTRTV" ;
                                                      <http://www.w3.org/2004/02/skos/core#definition> "Describes vehicle used for treatment. Example: SALINE." ;
                                                      <http://www.w3.org/2004/02/skos/core#exactMatch> "Thesaurus:C83292 (http://ncicb.nci.nih.gov/xml/owl/EVS/Thesaurus.owl#C83292)" .


###  https://purls.helmholtz-metadaten.de/ptroDKFZ000013
<https://purls.helmholtz-metadaten.de/ptroDKFZ000013> rdf:type owl:DatatypeProperty ;
                                                      rdfs:domain <http://ncicb.nci.nih.gov/xml/owl/EVS/Thesaurus.owl#C69256> ;
                                                      rdfs:range xsd:string ;
                                                      <http://purl.org/dc/elements/1.1/creator> "OGiraldo" ;
                                                      rdfs:isDefinedBy "https://library.cdisc.org/browser" ;
                                                      rdfs:label "Name_of_Actual_Treatment" ;
                                                      <http://www.w3.org/2004/02/skos/core#altLabel> "EXTRT" ;
                                                      <http://www.w3.org/2004/02/skos/core#definition> "Name of the treatment, as defined by the protocol." ;
                                                      <http://www.w3.org/2004/02/skos/core#exactMatch> "Thesaurus:C83091 (http://ncicb.nci.nih.gov/xml/owl/EVS/Thesaurus.owl#C83091)" .


###  https://purls.helmholtz-metadaten.de/ptroDKFZ000015
<https://purls.helmholtz-metadaten.de/ptroDKFZ000015> rdf:type owl:DatatypeProperty ;
                                                      rdfs:domain <http://ncicb.nci.nih.gov/xml/owl/EVS/Thesaurus.owl#C69256> ;
                                                      rdfs:range xsd:string ;
                                                      <http://purl.org/dc/elements/1.1/creator> "OGiraldo" ;
                                                      rdfs:isDefinedBy "https://library.cdisc.org/browser" ;
                                                      rdfs:label "Body_Weight_Test_Short_Name" ;
                                                      <http://www.w3.org/2004/02/skos/core#altLabel> "BWTESTCD" ;
                                                      <http://www.w3.org/2004/02/skos/core#definition> "Short name of the measurement, test, or examination described in BWTEST. It can be used as a column name when converting a dataset from a vertical to a horizontal format. The value in BWTESTCD cannot be longer than 8 characters, nor can it start with a number (e.g., \"1TEST\" is not valid). BWTESTCD cannot contain characters other than letters, numbers, or underscores." ;
                                                      <http://www.w3.org/2004/02/skos/core#exactMatch> "Thesaurus:C119795 (http://ncicb.nci.nih.gov/xml/owl/EVS/Thesaurus.owl#C119795)" .


###  https://purls.helmholtz-metadaten.de/ptroDKFZ000016
<https://purls.helmholtz-metadaten.de/ptroDKFZ000016> rdf:type owl:DatatypeProperty ;
                                                      rdfs:domain <http://ncicb.nci.nih.gov/xml/owl/EVS/Thesaurus.owl#C69256> ;
                                                      rdfs:range xsd:string ;
                                                      <http://purl.org/dc/elements/1.1/creator> "OGiraldo" ;
                                                      rdfs:isDefinedBy "https://library.cdisc.org/browser" ;
                                                      rdfs:label "Body_Weight_Test_Name" ;
                                                      <http://www.w3.org/2004/02/skos/core#altLabel> "BWTEST" ;
                                                      <http://www.w3.org/2004/02/skos/core#definition> "Long name for BWTESTCD. The value in BWTEST cannot be longer than 40 characters." ;
                                                      <http://www.w3.org/2004/02/skos/core#exactMatch> "Thesaurus:C119794 (http://ncicb.nci.nih.gov/xml/owl/EVS/Thesaurus.owl#C119794)" .


###  https://purls.helmholtz-metadaten.de/ptroDKFZ000017
<https://purls.helmholtz-metadaten.de/ptroDKFZ000017> rdf:type owl:DatatypeProperty ;
                                                      rdfs:domain <http://ncicb.nci.nih.gov/xml/owl/EVS/Thesaurus.owl#C69256> ;
                                                      rdfs:range xsd:decimal ;
                                                      <http://purl.org/dc/elements/1.1/creator> "OGiraldo" ;
                                                      rdfs:isDefinedBy "https://library.cdisc.org/browser" ;
                                                      rdfs:label "Body_Weight_Result_or_Findings_as_Collected" ;
                                                      <http://www.w3.org/2004/02/skos/core#altLabel> "BWORRES" ;
                                                      <http://www.w3.org/2004/02/skos/core#definition> "Result of the measurement or finding as originally received or collected." ;
                                                      <http://www.w3.org/2004/02/skos/core#exactMatch> "Thesaurus:C119785 (http://ncicb.nci.nih.gov/xml/owl/EVS/Thesaurus.owl#C119785)" .


###  https://purls.helmholtz-metadaten.de/ptroDKFZ000018
<https://purls.helmholtz-metadaten.de/ptroDKFZ000018> rdf:type owl:DatatypeProperty ;
                                                      rdfs:domain <http://ncicb.nci.nih.gov/xml/owl/EVS/Thesaurus.owl#C69256> ;
                                                      rdfs:range xsd:decimal ;
                                                      <http://purl.org/dc/elements/1.1/creator> "OGiraldo" ;
                                                      rdfs:isDefinedBy "https://library.cdisc.org/browser" ;
                                                      rdfs:label "Study_Day_Animal_Weighed" ;
                                                      <http://www.w3.org/2004/02/skos/core#altLabel> "BWDY" ;
                                                      <http://www.w3.org/2004/02/skos/core#definition> "Study day of body weight collection, in integer days. The algorithm for calculations must be relative to the sponsor-defined RFSTDTC variable in the Demographics (DM) domain." ;
                                                      <http://www.w3.org/2004/02/skos/core#exactMatch> "Thesaurus:C119782 (http://ncicb.nci.nih.gov/xml/owl/EVS/Thesaurus.owl#C119782)" .


###  https://purls.helmholtz-metadaten.de/ptroDKFZ000019
<https://purls.helmholtz-metadaten.de/ptroDKFZ000019> rdf:type owl:DatatypeProperty ;
                                                      rdfs:domain <http://ncicb.nci.nih.gov/xml/owl/EVS/Thesaurus.owl#C69256> ;
                                                      rdfs:range xsd:string ;
                                                      <http://purl.org/dc/elements/1.1/creator> "OGiraldo" ;
                                                      rdfs:isDefinedBy "https://library.cdisc.org/browser" ;
                                                      rdfs:label "Death_Diagnosis_Short_Name" ;
                                                      <http://www.w3.org/2004/02/skos/core#altLabel> "DDTESTCD" ;
                                                      <http://www.w3.org/2004/02/skos/core#definition> "Short name of the measurement, test, or examination described in DDTEST. It can be used as a column name when converting a dataset from a vertical to a horizontal format. The value in DDTESTCD cannot be longer than 8 characters, nor can it start with a number (e.g., \"1TEST\" is not valid). DDTESTCD cannot contain characters other than letters, numbers, or underscores." ;
                                                      <http://www.w3.org/2004/02/skos/core#exactMatch> "Thesaurus:C89966 (http://ncicb.nci.nih.gov/xml/owl/EVS/Thesaurus.owl#C89966)" .


###  https://purls.helmholtz-metadaten.de/ptroDKFZ000020
<https://purls.helmholtz-metadaten.de/ptroDKFZ000020> rdf:type owl:DatatypeProperty ;
                                                      rdfs:domain <http://ncicb.nci.nih.gov/xml/owl/EVS/Thesaurus.owl#C69256> ;
                                                      rdfs:range xsd:string ;
                                                      <http://purl.org/dc/elements/1.1/creator> "OGiraldo" ;
                                                      rdfs:isDefinedBy "https://library.cdisc.org/browser" ;
                                                      rdfs:label "Death_Diagnosis_Name" ;
                                                      <http://www.w3.org/2004/02/skos/core#altLabel> "DDTEST" ;
                                                      <http://www.w3.org/2004/02/skos/core#definition> "Long name for DDTESTCD. The value in DDTEST cannot be longer than 40 characters." ;
                                                      <http://www.w3.org/2004/02/skos/core#exactMatch> "Thesaurus:C89965 (http://ncicb.nci.nih.gov/xml/owl/EVS/Thesaurus.owl#C89965)" .


###  https://purls.helmholtz-metadaten.de/ptroDKFZ000021
<https://purls.helmholtz-metadaten.de/ptroDKFZ000021> rdf:type owl:DatatypeProperty ;
                                                      rdfs:domain <http://ncicb.nci.nih.gov/xml/owl/EVS/Thesaurus.owl#C69256> ;
                                                      rdfs:range xsd:string ;
                                                      <http://purl.org/dc/elements/1.1/creator> "OGiraldo" ;
                                                      rdfs:isDefinedBy "https://library.cdisc.org/browser" ;
                                                      rdfs:label "Death_Diagnosis_Result_Category" ;
                                                      <http://www.w3.org/2004/02/skos/core#altLabel> "DDRESCAT" ;
                                                      <http://www.w3.org/2004/02/skos/core#definition> "Used to categorize the result of a finding. Examples: TREATMENT RELATED, NONTREATMENT RELATED, UNDETERMINED, ACCIDENTAL, etc." ;
                                                      <http://www.w3.org/2004/02/skos/core#exactMatch> "Thesaurus:C102742 (http://ncicb.nci.nih.gov/xml/owl/EVS/Thesaurus.owl#C102742)" .


###  https://purls.helmholtz-metadaten.de/ptroDKFZ000022
<https://purls.helmholtz-metadaten.de/ptroDKFZ000022> rdf:type owl:DatatypeProperty ;
                                                      rdfs:domain <http://ncicb.nci.nih.gov/xml/owl/EVS/Thesaurus.owl#C69256> ;
                                                      rdfs:range xsd:string ;
                                                      <http://purl.org/dc/elements/1.1/creator> "OGiraldo" ;
                                                      rdfs:isDefinedBy "https://library.cdisc.org/browser" ;
                                                      rdfs:label "Death_Diagnosis_Evaluator" ;
                                                      <http://www.w3.org/2004/02/skos/core#altLabel> "DDEVAL" ;
                                                      <http://www.w3.org/2004/02/skos/core#definition> "Role of the person who provided the evaluation. Examples: TOX PATHOLOGIST, PEER REVIEW, SPONSOR, VETERINARIAN." ;
                                                      <http://www.w3.org/2004/02/skos/core#exactMatch> "Thesaurus:C117548 (http://ncicb.nci.nih.gov/xml/owl/EVS/Thesaurus.owl#C117548)" .


###  https://purls.helmholtz-metadaten.de/ptroDKFZ000023
<https://purls.helmholtz-metadaten.de/ptroDKFZ000023> rdf:type owl:DatatypeProperty ;
                                                      rdfs:domain <http://ncicb.nci.nih.gov/xml/owl/EVS/Thesaurus.owl#C69256> ;
                                                      rdfs:range xsd:string ;
                                                      <http://purl.org/dc/elements/1.1/creator> "OGiraldo" ;
                                                      rdfs:comment "a.k.a study day in CDISC" ;
                                                      rdfs:isDefinedBy "https://library.cdisc.org/browser" ;
                                                      rdfs:label "Study_day_Animal_Death" ;
                                                      <http://www.w3.org/2004/02/skos/core#altLabel> "DDDY" ;
                                                      <http://www.w3.org/2004/02/skos/core#definition> "Study day of subject disposition, in integer days. The algorithm for calculations must be relative to the sponsor-defined RFSTDTC variable in the Demographics (DM) domain." ;
                                                      <http://www.w3.org/2004/02/skos/core#exactMatch> "Thesaurus:C117550 (http://ncicb.nci.nih.gov/xml/owl/EVS/Thesaurus.owl#C117550)" .


###  https://purls.helmholtz-metadaten.de/ptroDKFZ000028
<https://purls.helmholtz-metadaten.de/ptroDKFZ000028> rdf:type owl:DatatypeProperty ;
                                                      rdfs:domain <http://ncicb.nci.nih.gov/xml/owl/EVS/Thesaurus.owl#C69256> ;
                                                      rdfs:range xsd:string ;
                                                      <http://purl.org/dc/elements/1.1/creator> "OGiraldo" ;
                                                      rdfs:isDefinedBy "https://library.cdisc.org/browser" ;
                                                      rdfs:label "Clinical_Observations_Test_Short_Name" ;
                                                      <http://www.w3.org/2004/02/skos/core#altLabel> "CLTESTCD" ;
                                                      <http://www.w3.org/2004/02/skos/core#definition> "Short name of the measurement, test, or examination described in CLTEST. It can be used as a column name when converting a dataset from a vertical to a horizontal format. The value in CLTESTCD cannot be longer than 8 characters, nor can it start with a number (e.g., \"1TEST\" is not valid). CLTESTCD cannot contain characters other than letters, numbers, or underscores." ;
                                                      <http://www.w3.org/2004/02/skos/core#exactMatch> "Thesaurus:C119815 (http://ncicb.nci.nih.gov/xml/owl/EVS/Thesaurus.owl#C119815)" .


###  https://purls.helmholtz-metadaten.de/ptroDKFZ000029
<https://purls.helmholtz-metadaten.de/ptroDKFZ000029> rdf:type owl:DatatypeProperty ;
                                                      rdfs:domain <http://ncicb.nci.nih.gov/xml/owl/EVS/Thesaurus.owl#C69256> ;
                                                      rdfs:range xsd:string ;
                                                      <http://purl.org/dc/elements/1.1/creator> "OGiraldo" ;
                                                      rdfs:isDefinedBy "https://library.cdisc.org/browser" ;
                                                      rdfs:label "Clinical_Observations_Test_Name" ;
                                                      <http://www.w3.org/2004/02/skos/core#altLabel> "CLTEST" ;
                                                      <http://www.w3.org/2004/02/skos/core#definition> "Long name for CLTESTCD. The value in CLTEST cannot be longer than 40 characters." ;
                                                      <http://www.w3.org/2004/02/skos/core#exactMatch> "Thesaurus:C119814 (http://ncicb.nci.nih.gov/xml/owl/EVS/Thesaurus.owl#C119814)" .


###  https://purls.helmholtz-metadaten.de/ptroDKFZ000030
<https://purls.helmholtz-metadaten.de/ptroDKFZ000030> rdf:type owl:DatatypeProperty ;
                                                      rdfs:domain <http://ncicb.nci.nih.gov/xml/owl/EVS/Thesaurus.owl#C69256> ;
                                                      rdfs:range xsd:string ;
                                                      <http://purl.org/dc/elements/1.1/creator> "OGiraldo" ;
                                                      rdfs:isDefinedBy "https://library.cdisc.org/browser" ;
                                                      rdfs:label "Category_for_Clinical_Observations" ;
                                                      <http://www.w3.org/2004/02/skos/core#altLabel> "CLCAT" ;
                                                      <http://www.w3.org/2004/02/skos/core#definition> "Used to define a category of the clinical observation." ;
                                                      <http://www.w3.org/2004/02/skos/core#exactMatch> "Thesaurus:C119797 (http://ncicb.nci.nih.gov/xml/owl/EVS/Thesaurus.owl#C119797)" .


###  https://purls.helmholtz-metadaten.de/ptroDKFZ000031
<https://purls.helmholtz-metadaten.de/ptroDKFZ000031> rdf:type owl:DatatypeProperty ;
                                                      rdfs:domain <http://ncicb.nci.nih.gov/xml/owl/EVS/Thesaurus.owl#C69256> ;
                                                      rdfs:range xsd:string ;
                                                      <http://purl.org/dc/elements/1.1/creator> "OGiraldo" ;
                                                      rdfs:isDefinedBy "https://library.cdisc.org/browser" ;
                                                      rdfs:label "Subcategory_for_Clinical_Observations" ;
                                                      <http://www.w3.org/2004/02/skos/core#altLabel> "CLSCAT" ;
                                                      <http://www.w3.org/2004/02/skos/core#definition> "Used to further categorize a group of clinical observations within a category. For example \"Whole Body Appearance\" and \"Sensory Organ Appearance\" may be subcategories within Clinical Signs." ;
                                                      <http://www.w3.org/2004/02/skos/core#exactMatch> "Thesaurus:C102740 (http://ncicb.nci.nih.gov/xml/owl/EVS/Thesaurus.owl#C102740)" .


###  https://purls.helmholtz-metadaten.de/ptroDKFZ000033
<https://purls.helmholtz-metadaten.de/ptroDKFZ000033> rdf:type owl:DatatypeProperty ;
                                                      rdfs:domain <http://ncicb.nci.nih.gov/xml/owl/EVS/Thesaurus.owl#C69256> ;
                                                      rdfs:range xsd:decimal ;
                                                      <http://purl.org/dc/elements/1.1/creator> "OGiraldo" ;
                                                      rdfs:isDefinedBy "https://library.cdisc.org/browser" ;
                                                      rdfs:label "Age" ;
                                                      <http://www.w3.org/2004/02/skos/core#altLabel> "AGE" ;
                                                      <http://www.w3.org/2004/02/skos/core#definition> "May be derived (RFSTDTC - BRTHDTC), but BRTHDTC may not be available in all cases. Age may also be collected." ;
                                                      <http://www.w3.org/2004/02/skos/core#exactMatch> "Thesaurus:C25150 (http://ncicb.nci.nih.gov/xml/owl/EVS/Thesaurus.owl#C25150)" .


###  https://purls.helmholtz-metadaten.de/ptroDKFZ000034
<https://purls.helmholtz-metadaten.de/ptroDKFZ000034> rdf:type owl:DatatypeProperty ;
                                                      rdfs:domain <http://ncicb.nci.nih.gov/xml/owl/EVS/Thesaurus.owl#C69256> ;
                                                      rdfs:range xsd:string ;
                                                      <http://purl.org/dc/elements/1.1/creator> "OGiraldo" ;
                                                      rdfs:isDefinedBy "https://library.cdisc.org/browser" ;
                                                      rdfs:label "Age_Unit" ;
                                                      <http://www.w3.org/2004/02/skos/core#altLabel> "AGEU" ;
                                                      <http://www.w3.org/2004/02/skos/core#definition> "Units associated with AGE and AGETXT." ;
                                                      <http://www.w3.org/2004/02/skos/core#exactMatch> "Thesaurus:C50400 (http://ncicb.nci.nih.gov/xml/owl/EVS/Thesaurus.owl#C50400)" .


###  https://purls.helmholtz-metadaten.de/ptroDKFZ000035
<https://purls.helmholtz-metadaten.de/ptroDKFZ000035> rdf:type owl:DatatypeProperty ;
                                                      rdfs:domain <http://ncicb.nci.nih.gov/xml/owl/EVS/Thesaurus.owl#C69256> ;
                                                      rdfs:range xsd:string ;
                                                      <http://purl.org/dc/elements/1.1/creator> "OGiraldo" ;
                                                      rdfs:isDefinedBy "https://library.cdisc.org/browser" ;
                                                      rdfs:label "Body_System_or_Organ_Class" ;
                                                      <http://www.w3.org/2004/02/skos/core#altLabel> "CLBODSYS" ;
                                                      <http://www.w3.org/2004/02/skos/core#definition> "Body system or organ class associated with the measurement performed." ;
                                                      <http://www.w3.org/2004/02/skos/core#exactMatch> "Thesaurus:C119796 (http://ncicb.nci.nih.gov/xml/owl/EVS/Thesaurus.owl#C119796)" .


###  https://purls.helmholtz-metadaten.de/ptroDKFZ000036
<https://purls.helmholtz-metadaten.de/ptroDKFZ000036> rdf:type owl:DatatypeProperty ;
                                                      rdfs:domain <http://ncicb.nci.nih.gov/xml/owl/EVS/Thesaurus.owl#C69256> ;
                                                      rdfs:range xsd:string ;
                                                      <http://purl.org/dc/elements/1.1/creator> "OGiraldo" ;
                                                      rdfs:isDefinedBy "https://library.cdisc.org/browser" ;
                                                      rdfs:label "Clinical_Observations_Result_Category" ;
                                                      <http://www.w3.org/2004/02/skos/core#altLabel> "CLRESCAT" ;
                                                      <http://www.w3.org/2004/02/skos/core#definition> "Used to categorize the result of a finding post collection. Examples: Color or Facial." ;
                                                      <http://www.w3.org/2004/02/skos/core#exactMatch> "Thesaurus:C102741 (http://ncicb.nci.nih.gov/xml/owl/EVS/Thesaurus.owl#C102741)" .


###  https://purls.helmholtz-metadaten.de/ptroDKFZ000037
<https://purls.helmholtz-metadaten.de/ptroDKFZ000037> rdf:type owl:DatatypeProperty ;
                                                      rdfs:domain <http://ncicb.nci.nih.gov/xml/owl/EVS/Thesaurus.owl#C69256> ;
                                                      rdfs:range xsd:string ;
                                                      <http://purl.org/dc/elements/1.1/creator> "OGiraldo" ;
                                                      rdfs:isDefinedBy "https://library.cdisc.org/browser" ;
                                                      rdfs:label "Clinical_Observations_Completion_Status" ;
                                                      <http://www.w3.org/2004/02/skos/core#altLabel> "CLSTAT" ;
                                                      <http://www.w3.org/2004/02/skos/core#definition> "Used to indicate examination not done or result is missing. Should be null if a result exists in CLORRES." ;
                                                      <http://www.w3.org/2004/02/skos/core#exactMatch> "Thesaurus:C119812 (http://ncicb.nci.nih.gov/xml/owl/EVS/Thesaurus.owl#C119812)" .


###  https://purls.helmholtz-metadaten.de/ptroDKFZ000038
<https://purls.helmholtz-metadaten.de/ptroDKFZ000038> rdf:type owl:DatatypeProperty ;
                                                      rdfs:domain <http://ncicb.nci.nih.gov/xml/owl/EVS/Thesaurus.owl#C69256> ;
                                                      rdfs:range xsd:string ;
                                                      <http://purl.org/dc/elements/1.1/creator> "OGiraldo" ;
                                                      rdfs:isDefinedBy "https://library.cdisc.org/browser" ;
                                                      rdfs:label "Clinical_Observations_Evaluator" ;
                                                      <http://www.w3.org/2004/02/skos/core#altLabel> "CLEVAL" ;
                                                      <http://www.w3.org/2004/02/skos/core#definition> "Role of the person who provided the evaluation. Example: TOX TECHNICIAN, OPHTHALMOLOGIST, VETERINARIAN." ;
                                                      <http://www.w3.org/2004/02/skos/core#exactMatch> "Thesaurus:C119801 (http://ncicb.nci.nih.gov/xml/owl/EVS/Thesaurus.owl#C119801)" .


###  https://purls.helmholtz-metadaten.de/ptroDKFZ000039
<https://purls.helmholtz-metadaten.de/ptroDKFZ000039> rdf:type owl:DatatypeProperty ;
                                                      rdfs:domain <http://ncicb.nci.nih.gov/xml/owl/EVS/Thesaurus.owl#C69256> ;
                                                      rdfs:range xsd:decimal ;
                                                      <http://purl.org/dc/elements/1.1/creator> "OGiraldo" ;
                                                      rdfs:isDefinedBy "https://library.cdisc.org/browser" ;
                                                      rdfs:label "Study_Day_of_Clinical_Observation" ;
                                                      <http://www.w3.org/2004/02/skos/core#altLabel> "CLDY" ;
                                                      <http://www.w3.org/2004/02/skos/core#definition> "Study day of observation, in integer days. For measurements related to a continuous evaluation interval, CLDY can be used to indicate start day of that interval. The algorithm for calculations must be relative to the sponsor-defined RFSTDTC variable in the Demographics (DM) domain." ;
                                                      <http://www.w3.org/2004/02/skos/core#exactMatch> "Thesaurus:C119799 (http://ncicb.nci.nih.gov/xml/owl/EVS/Thesaurus.owl#C119799)" .


###  https://purls.helmholtz-metadaten.de/ptroDKFZ000040
<https://purls.helmholtz-metadaten.de/ptroDKFZ000040> rdf:type owl:DatatypeProperty ;
                                                      rdfs:domain <http://ncicb.nci.nih.gov/xml/owl/EVS/Thesaurus.owl#C69256> ;
                                                      rdfs:range xsd:integer ;
                                                      <http://purl.org/dc/elements/1.1/creator> "OGiraldo" ;
                                                      rdfs:isDefinedBy "https://library.cdisc.org/browser" ;
                                                      rdfs:label "Sex" ;
                                                      <http://www.w3.org/2004/02/skos/core#altLabel> "SEX" ;
                                                      <http://www.w3.org/2004/02/skos/core#definition> "The sex of the subject." ;
                                                      <http://www.w3.org/2004/02/skos/core#exactMatch> "Thesaurus:C28421 (http://ncicb.nci.nih.gov/xml/owl/EVS/Thesaurus.owl#C28421)" .


###  https://purls.helmholtz-metadaten.de/ptroDKFZ000041
<https://purls.helmholtz-metadaten.de/ptroDKFZ000041> rdf:type owl:DatatypeProperty ;
                                                      rdfs:domain <http://ncicb.nci.nih.gov/xml/owl/EVS/Thesaurus.owl#C69256> ;
                                                      rdfs:range xsd:string ;
                                                      <http://purl.org/dc/elements/1.1/creator> "OGiraldo" ;
                                                      rdfs:isDefinedBy "https://library.cdisc.org/browser" ;
                                                      rdfs:label "Strain_Substrain" ;
                                                      <http://www.w3.org/2004/02/skos/core#altLabel> "STRAIN" ;
                                                      <http://www.w3.org/2004/02/skos/core#definition> "Used to identify the vendor-supplied strain, substrain, or breed designation for the test system under study. It may combine the background strain, substrain, and associated genetic modifications as supplied by the vendor (e.g., C57BL/6, A/J, B6.129-Pparg<tm2Rev>/J, FISCHER 344, SPRAGUE-DAWLEY IGS, WISTAR Kyoto, BEAGLE, CYNOMOLGUS, and CHIMPANZEE). The SEND Controlled Terminology codelist consists of commonly used wild type strains. It is extensible to accommodate strains not listed and genetically modified substrains. If this variable is excluded in the DM domain, the information must be present at a higher level (either Trial Sets or Trial Summary). Country of origin for non-human primates should not go into STRAIN. In general, details related to coat color (e.g., White and Red designations for New Zealand Rabbits) should not go into STRAIN." ;
                                                      <http://www.w3.org/2004/02/skos/core#exactMatch> "Thesaurus:C96373 (http://ncicb.nci.nih.gov/xml/owl/EVS/Thesaurus.owl#C96373)" .


###  https://purls.helmholtz-metadaten.de/ptroDKFZ000042
<https://purls.helmholtz-metadaten.de/ptroDKFZ000042> rdf:type owl:DatatypeProperty ;
                                                      rdfs:domain <http://ncicb.nci.nih.gov/xml/owl/EVS/Thesaurus.owl#C69256> ;
                                                      rdfs:range xsd:string ;
                                                      <http://purl.org/dc/elements/1.1/creator> "OGiraldo" ;
                                                      rdfs:isDefinedBy "https://library.cdisc.org/browser" ;
                                                      rdfs:label "Domain_Abbreviation" ;
                                                      <http://www.w3.org/2004/02/skos/core#altLabel> "DOMAIN" ;
                                                      <http://www.w3.org/2004/02/skos/core#definition> "Two-character abbreviation for the domain." .


###  https://purls.helmholtz-metadaten.de/ptroDKFZ000043
<https://purls.helmholtz-metadaten.de/ptroDKFZ000043> rdf:type owl:DatatypeProperty ;
                                                      rdfs:domain <http://ncicb.nci.nih.gov/xml/owl/EVS/Thesaurus.owl#C69256> ;
                                                      rdfs:range xsd:string ;
                                                      <http://purl.org/dc/elements/1.1/creator> "OGiraldo" ;
                                                      rdfs:isDefinedBy "https://library.cdisc.org/browser" ;
                                                      rdfs:label "Age_Range" ;
                                                      <http://www.w3.org/2004/02/skos/core#altLabel> "AGETXT" ;
                                                      <http://www.w3.org/2004/02/skos/core#definition> "Used when the age is a range and the exact birthdate is not known. This variable is a character field for the purposes of defining age ranges, e.g., if the information available for the age of the subject is 6-8 and AGEU is WEEKS. Populate only when BRTHDTC or AGE is not specified. The format for AGETXT is \"number-number\" (e.g., 6-8)." ;
                                                      <http://www.w3.org/2004/02/skos/core#exactMatch> "Thesaurus:C90352 (http://ncicb.nci.nih.gov/xml/owl/EVS/Thesaurus.owl#C90352)" .


###  https://purls.helmholtz-metadaten.de/ptroDKFZ000044
<https://purls.helmholtz-metadaten.de/ptroDKFZ000044> rdf:type owl:DatatypeProperty ;
                                                      rdfs:domain <http://ncicb.nci.nih.gov/xml/owl/EVS/Thesaurus.owl#C69256> ;
                                                      rdfs:range xsd:decimal ;
                                                      <http://purl.org/dc/elements/1.1/creator> "OGiraldo" ;
                                                      rdfs:isDefinedBy "https://library.cdisc.org/browser" ;
                                                      rdfs:label "Study_Day_of_Start_of_Treatment" ;
                                                      <http://www.w3.org/2004/02/skos/core#altLabel> "EXSTDY" ;
                                                      <http://www.w3.org/2004/02/skos/core#definition> "Study day when administration of the treatment began, in integer days. The algorithm for calculations must be relative to the sponsor-defined RFSTDTC variable in the Demographics (DM) domain." ;
                                                      <http://www.w3.org/2004/02/skos/core#exactMatch> "Thesaurus:C83289 (http://ncicb.nci.nih.gov/xml/owl/EVS/Thesaurus.owl#C83289)" .


###  https://purls.helmholtz-metadaten.de/ptroDKFZ000046
<https://purls.helmholtz-metadaten.de/ptroDKFZ000046> rdf:type owl:DatatypeProperty ;
                                                      rdfs:domain <http://ncicb.nci.nih.gov/xml/owl/EVS/Thesaurus.owl#C69256> ;
                                                      rdfs:range xsd:string ;
                                                      <http://purl.org/dc/elements/1.1/creator> "OGiraldo" ;
                                                      rdfs:comment "a.k.a Unit of the Original Result in CDISC Data Standards Browser" ;
                                                      rdfs:label "Body_Weight_Unit_of_the_Original_Result" ;
                                                      <http://www.w3.org/2004/02/skos/core#altLabel> "BWORRESU" ;
                                                      <http://www.w3.org/2004/02/skos/core#definition> "The unit for the original result. The unit of the original result should be mapped to a synonymous unit on the Controlled Terminology list." ;
                                                      <http://www.w3.org/2004/02/skos/core#exactMatch> "Thesaurus:C119786 (http://ncicb.nci.nih.gov/xml/owl/EVS/Thesaurus.owl#C119786)" .


###  https://purls.helmholtz-metadaten.de/ptroDKFZ000051
<https://purls.helmholtz-metadaten.de/ptroDKFZ000051> rdf:type owl:DatatypeProperty ;
                                                      rdfs:domain <http://ncicb.nci.nih.gov/xml/owl/EVS/Thesaurus.owl#C69256> ;
                                                      rdfs:range xsd:string ;
                                                      <http://purl.org/dc/elements/1.1/creator> "OGiraldo" ;
                                                      rdfs:label "Session_Identifier" ;
                                                      <http://www.w3.org/2004/02/skos/core#definition> "Session identifier used within the EX template." .


###  https://purls.helmholtz-metadaten.de/ptroDKFZ000053
<https://purls.helmholtz-metadaten.de/ptroDKFZ000053> rdf:type owl:DatatypeProperty ;
                                                      rdfs:domain <http://ncicb.nci.nih.gov/xml/owl/EVS/Thesaurus.owl#C69256> ;
                                                      rdfs:range xsd:decimal ;
                                                      <http://purl.org/dc/elements/1.1/creator> "OGiraldo" ;
                                                      rdfs:isDefinedBy "https://library.cdisc.org/browser" ;
                                                      rdfs:label "Exposure_Dose_per_Administration" ;
                                                      <http://www.w3.org/2004/02/skos/core#altLabel> "EXDOSE" ;
                                                      <http://www.w3.org/2004/02/skos/core#definition> "Amount of treatment administered." ;
                                                      <http://www.w3.org/2004/02/skos/core#exactMatch> "Thesaurus:C83039 (http://ncicb.nci.nih.gov/xml/owl/EVS/Thesaurus.owl#C83039)" .


###  https://purls.helmholtz-metadaten.de/ptroDKFZ000054
<https://purls.helmholtz-metadaten.de/ptroDKFZ000054> rdf:type owl:DatatypeProperty ;
                                                      rdfs:domain <http://ncicb.nci.nih.gov/xml/owl/EVS/Thesaurus.owl#C69256> ;
                                                      rdfs:range xsd:string ;
                                                      <http://purl.org/dc/elements/1.1/creator> "OGiraldo" ;
                                                      rdfs:isDefinedBy "https://library.cdisc.org/browser" ;
                                                      rdfs:label "Exposure_Dose_Units" ;
                                                      <http://www.w3.org/2004/02/skos/core#altLabel> "EXDOSU" ;
                                                      <http://www.w3.org/2004/02/skos/core#definition> "Units for EXDOSE or EXDOSTXT. Examples: ng, mg, or mg/kg." ;
                                                      <http://www.w3.org/2004/02/skos/core#exactMatch> "Thesaurus:C83035 (http://ncicb.nci.nih.gov/xml/owl/EVS/Thesaurus.owl#C83035)" .


###  https://purls.helmholtz-metadaten.de/ptroDKFZ000055
<https://purls.helmholtz-metadaten.de/ptroDKFZ000055> rdf:type owl:DatatypeProperty ;
                                                      rdfs:domain <http://ncicb.nci.nih.gov/xml/owl/EVS/Thesaurus.owl#C69256> ;
                                                      rdfs:range xsd:decimal ;
                                                      <http://purl.org/dc/elements/1.1/creator> "OGiraldo" ;
                                                      rdfs:isDefinedBy "https://library.cdisc.org/browser" ;
                                                      rdfs:label "Amount_Administered" ;
                                                      <http://www.w3.org/2004/02/skos/core#altLabel> "EXVAMT" ;
                                                      <http://www.w3.org/2004/02/skos/core#definition> "The amount (volume or weight) of the treatment compound plus vehicle administered in a single dose. This is not to be confused with EXDOSE. EXDOSE refers to the amount of test material administered to the subject." ;
                                                      <http://www.w3.org/2004/02/skos/core#exactMatch> "Thesaurus:C87883 (http://ncicb.nci.nih.gov/xml/owl/EVS/Thesaurus.owl#C87883)" .


###  https://purls.helmholtz-metadaten.de/ptroDKFZ000056
<https://purls.helmholtz-metadaten.de/ptroDKFZ000056> rdf:type owl:DatatypeProperty ;
                                                      rdfs:domain <http://ncicb.nci.nih.gov/xml/owl/EVS/Thesaurus.owl#C69256> ;
                                                      rdfs:range xsd:string ;
                                                      <http://purl.org/dc/elements/1.1/creator> "OGiraldo" ;
                                                      rdfs:isDefinedBy "https://library.cdisc.org/browser" ;
                                                      rdfs:label "Amount_Administered_Units" ;
                                                      <http://www.w3.org/2004/02/skos/core#altLabel> "EXVAMTU" ;
                                                      <http://www.w3.org/2004/02/skos/core#definition> "Units for EXVAMT (per dose administration)." ;
                                                      <http://www.w3.org/2004/02/skos/core#exactMatch> "Thesaurus:C87884 (http://ncicb.nci.nih.gov/xml/owl/EVS/Thesaurus.owl#C87884)" .


###  https://purls.helmholtz-metadaten.de/ptroDKFZ000057
<https://purls.helmholtz-metadaten.de/ptroDKFZ000057> rdf:type owl:DatatypeProperty ;
                                                      rdfs:domain <http://ncicb.nci.nih.gov/xml/owl/EVS/Thesaurus.owl#C69256> ;
                                                      rdfs:range xsd:decimal ;
                                                      <http://purl.org/dc/elements/1.1/creator> "OGiraldo" ;
                                                      rdfs:isDefinedBy "https://library.cdisc.org/browser" ;
                                                      rdfs:label "Study_Day_of_End_Date_of_Treatment" ;
                                                      <http://www.w3.org/2004/02/skos/core#altLabel> "EXENDY" ;
                                                      <http://www.w3.org/2004/02/skos/core#definition> "Study day when administration of the treatment ended, in integer days. The algorithm for calculations must be relative to the sponsor-defined RFSTDTC variable in the Demographics (DM) domain." ;
                                                      <http://www.w3.org/2004/02/skos/core#exactMatch> "Thesaurus:C83283 (http://ncicb.nci.nih.gov/xml/owl/EVS/Thesaurus.owl#C83283)" .


###  https://purls.helmholtz-metadaten.de/ptroDKFZ000058
<https://purls.helmholtz-metadaten.de/ptroDKFZ000058> rdf:type owl:DatatypeProperty ;
                                                      rdfs:domain <http://ncicb.nci.nih.gov/xml/owl/EVS/Thesaurus.owl#C69256> ;
                                                      rdfs:range xsd:decimal ;
                                                      <http://purl.org/dc/elements/1.1/creator> "OGiraldo" ;
                                                      rdfs:isDefinedBy "https://library.cdisc.org/browser" ;
                                                      rdfs:label "Duration_of_Treatment" ;
                                                      <http://www.w3.org/2004/02/skos/core#altLabel> "EXDUR" ;
                                                      <http://www.w3.org/2004/02/skos/core#definition> "Duration and unit of time for a continuous treatment. This may be used to denote the length of an infusion (e.g., PT10M to indicate 10 minutes)." ;
                                                      <http://www.w3.org/2004/02/skos/core#exactMatch> "Thesaurus:C83280 (http://ncicb.nci.nih.gov/xml/owl/EVS/Thesaurus.owl#C83280)" .


###  https://purls.helmholtz-metadaten.de/ptroDKFZ000060
<https://purls.helmholtz-metadaten.de/ptroDKFZ000060> rdf:type owl:DatatypeProperty ;
                                                      rdfs:domain <http://ncicb.nci.nih.gov/xml/owl/EVS/Thesaurus.owl#C69256> ;
                                                      rdfs:range xsd:string ;
                                                      <http://purl.org/dc/elements/1.1/creator> "OGiraldo" ;
                                                      rdfs:isDefinedBy "https://library.cdisc.org/browser" ;
                                                      rdfs:label "Lab_Test_or_Examination_Short_Name" ;
                                                      <http://www.w3.org/2004/02/skos/core#altLabel> "LBTESTCD" ;
                                                      <http://www.w3.org/2004/02/skos/core#definition> "Short name of the measurement, test, or examination described in LBTEST. It can be used as a column name when converting a dataset from a vertical to a horizontal format. The value in LBTESTCD cannot be longer than 8 characters, nor can it start with a number (e.g., \"1TEST\" is not valid). LBTESTCD cannot contain characters other than letters, numbers, or underscores. Examples: ALT, LDH." ;
                                                      <http://www.w3.org/2004/02/skos/core#exactMatch> "Thesaurus:C83322 (http://ncicb.nci.nih.gov/xml/owl/EVS/Thesaurus.owl#C83322)" .


###  https://purls.helmholtz-metadaten.de/ptroDKFZ000061
<https://purls.helmholtz-metadaten.de/ptroDKFZ000061> rdf:type owl:DatatypeProperty ;
                                                      rdfs:domain <http://ncicb.nci.nih.gov/xml/owl/EVS/Thesaurus.owl#C69256> ;
                                                      rdfs:range xsd:string ;
                                                      <http://purl.org/dc/elements/1.1/creator> "OGiraldo" ;
                                                      rdfs:isDefinedBy "https://library.cdisc.org/browser" ;
                                                      rdfs:label "Lab_Test_or_Examination_Name" ;
                                                      <http://www.w3.org/2004/02/skos/core#altLabel> "LBTEST" ;
                                                      <http://www.w3.org/2004/02/skos/core#definition> "Long name for LBTESTCD. The value in LBTEST cannot be longer than 40 characters. Examples: Alanine Aminotransferase, Lactate Dehydrogenase." .


###  https://purls.helmholtz-metadaten.de/ptroDKFZ000062
<https://purls.helmholtz-metadaten.de/ptroDKFZ000062> rdf:type owl:DatatypeProperty ;
                                                      rdfs:domain <http://ncicb.nci.nih.gov/xml/owl/EVS/Thesaurus.owl#C69256> ;
                                                      rdfs:range xsd:decimal ;
                                                      <http://purl.org/dc/elements/1.1/creator> "OGiraldo" ;
                                                      rdfs:isDefinedBy "https://library.cdisc.org/browser" ;
                                                      rdfs:label "Lab_Result_or_Findings_as_Collected" ;
                                                      <http://www.w3.org/2004/02/skos/core#altLabel> "LBORRES" ;
                                                      <http://www.w3.org/2004/02/skos/core#definition> "Result of the measurement or finding as originally received or collected." ;
                                                      <http://www.w3.org/2004/02/skos/core#exactMatch> "Thesaurus:C83165 (http://ncicb.nci.nih.gov/xml/owl/EVS/Thesaurus.owl#C83165)" .


###  https://purls.helmholtz-metadaten.de/ptroDKFZ000063
<https://purls.helmholtz-metadaten.de/ptroDKFZ000063> rdf:type owl:DatatypeProperty ;
                                                      rdfs:domain <http://ncicb.nci.nih.gov/xml/owl/EVS/Thesaurus.owl#C69256> ;
                                                      rdfs:range xsd:string ;
                                                      <http://purl.org/dc/elements/1.1/creator> "OGiraldo" ;
                                                      rdfs:isDefinedBy "https://library.cdisc.org/browser" ;
                                                      rdfs:label "Lab_Unit_of_the_Original_Result" ;
                                                      <http://www.w3.org/2004/02/skos/core#altLabel> "LBORRESU" ;
                                                      <http://www.w3.org/2004/02/skos/core#definition> "The unit for the original result. The unit of the original result should be mapped to a synonymous unit on the Controlled Terminology (http://www.cdisc.org/terminology) list." ;
                                                      <http://www.w3.org/2004/02/skos/core#exactMatch> "Thesaurus:C83106 (http://ncicb.nci.nih.gov/xml/owl/EVS/Thesaurus.owl#C83106)" .


###  https://purls.helmholtz-metadaten.de/ptroDKFZ000064
<https://purls.helmholtz-metadaten.de/ptroDKFZ000064> rdf:type owl:DatatypeProperty ;
                                                      rdfs:domain <http://ncicb.nci.nih.gov/xml/owl/EVS/Thesaurus.owl#C69256> ;
                                                      rdfs:range xsd:string ;
                                                      <http://purl.org/dc/elements/1.1/creator> "OGiraldo" ;
                                                      rdfs:isDefinedBy "https://library.cdisc.org/browser" ;
                                                      rdfs:label "Laboratory_Name" ;
                                                      <http://www.w3.org/2004/02/skos/core#altLabel> "LBNAM" ;
                                                      <http://www.w3.org/2004/02/skos/core#definition> "Name or identifier of the laboratory or vendor that provided the test results." .


###  https://purls.helmholtz-metadaten.de/ptroDKFZ000065
<https://purls.helmholtz-metadaten.de/ptroDKFZ000065> rdf:type owl:DatatypeProperty ;
                                                      rdfs:domain <http://ncicb.nci.nih.gov/xml/owl/EVS/Thesaurus.owl#C69256> ;
                                                      rdfs:range xsd:string ;
                                                      <http://purl.org/dc/elements/1.1/creator> "OGiraldo" ;
                                                      rdfs:isDefinedBy "https://library.cdisc.org/browser" ;
                                                      rdfs:label "Anatomical_Region_of_Specimen" ;
                                                      <http://www.w3.org/2004/02/skos/core#altLabel> "LBANTREG" ;
                                                      <http://www.w3.org/2004/02/skos/core#definition> "Defines the specific anatomical or biological region of a tissue, organ specimen, or the region from which the specimen was obtained, such as a section or part of what is defined in the LBSPEC variable. If the anatomical region is not included in the specimen description LBSPEC, it may be included in this variable. This field can be a combination of terms where needed. This field can be null if not applicable. Examples: CORTEX, MEDULLA, MUCOSA, SEROSA, ISLET, ZONA FASICULATA, ZONA RETICULARIS, CRANIAL, MEDIAN, ACCESSORY, SPINAL, LUMBAR, FRONTAL." ;
                                                      <http://www.w3.org/2004/02/skos/core#exactMatch> "Thesaurus:C119844 (http://ncicb.nci.nih.gov/xml/owl/EVS/Thesaurus.owl#C119844)" .


###  https://purls.helmholtz-metadaten.de/ptroDKFZ000066
<https://purls.helmholtz-metadaten.de/ptroDKFZ000066> rdf:type owl:DatatypeProperty ;
                                                      rdfs:domain <http://ncicb.nci.nih.gov/xml/owl/EVS/Thesaurus.owl#C69256> ;
                                                      rdfs:range xsd:string ;
                                                      <http://purl.org/dc/elements/1.1/creator> "OGiraldo" ;
                                                      rdfs:isDefinedBy "https://library.cdisc.org/browser" ;
                                                      rdfs:label "Specimen_Condition" ;
                                                      <http://www.w3.org/2004/02/skos/core#altLabel> "LBSPCCND" ;
                                                      <http://www.w3.org/2004/02/skos/core#definition> "Free or standardized text describing the condition of the specimen. Examples: HEMOLYZED, ICTERIC, LIPEMIC" ;
                                                      <http://www.w3.org/2004/02/skos/core#exactMatch> "Thesaurus:C83024 (http://ncicb.nci.nih.gov/xml/owl/EVS/Thesaurus.owl#C83024)" .


###  https://purls.helmholtz-metadaten.de/ptroDKFZ000067
<https://purls.helmholtz-metadaten.de/ptroDKFZ000067> rdf:type owl:DatatypeProperty ;
                                                      rdfs:domain <http://ncicb.nci.nih.gov/xml/owl/EVS/Thesaurus.owl#C69256> ;
                                                      rdfs:range xsd:string ;
                                                      <http://purl.org/dc/elements/1.1/creator> "OGiraldo" ;
                                                      rdfs:isDefinedBy "https://library.cdisc.org/browser" ;
                                                      rdfs:label "Specimen_Usability_for_the_Test" ;
                                                      <http://www.w3.org/2004/02/skos/core#altLabel> "LBSPCUFL" ;
                                                      <http://www.w3.org/2004/02/skos/core#definition> "Describes the usability of the specimen for the test. Should be N if the specimen is not usable; otherwise it should be null." ;
                                                      <http://www.w3.org/2004/02/skos/core#exactMatch> "Thesaurus:C119852 (http://ncicb.nci.nih.gov/xml/owl/EVS/Thesaurus.owl#C119852)" .


###  https://purls.helmholtz-metadaten.de/ptroDKFZ000068
<https://purls.helmholtz-metadaten.de/ptroDKFZ000068> rdf:type owl:DatatypeProperty ;
                                                      rdfs:domain <http://ncicb.nci.nih.gov/xml/owl/EVS/Thesaurus.owl#C69256> ;
                                                      rdfs:range xsd:string ;
                                                      <http://purl.org/dc/elements/1.1/creator> "OGiraldo" ;
                                                      rdfs:isDefinedBy "https://library.cdisc.org/browser" ;
                                                      rdfs:label "Lab_Portion_or_Totality" ;
                                                      <http://www.w3.org/2004/02/skos/core#altLabel> "LBPORTOT" ;
                                                      <http://www.w3.org/2004/02/skos/core#definition> "Qualifier for anatomical location or specimen further detailing the portion or totality, which means arrangement of, or apportioning of. Examples: ENTIRE, SINGLE, SEGMENT, MANY." ;
                                                      <http://www.w3.org/2004/02/skos/core#exactMatch> "Thesaurus:C119850 (http://ncicb.nci.nih.gov/xml/owl/EVS/Thesaurus.owl#C119850)" .


###  https://purls.helmholtz-metadaten.de/ptroDKFZ000069
<https://purls.helmholtz-metadaten.de/ptroDKFZ000069> rdf:type owl:DatatypeProperty ;
                                                      rdfs:domain <http://ncicb.nci.nih.gov/xml/owl/EVS/Thesaurus.owl#C69256> ;
                                                      rdfs:range xsd:string ;
                                                      <http://purl.org/dc/elements/1.1/creator> "OGiraldo" ;
                                                      rdfs:isDefinedBy "https://library.cdisc.org/browser" ;
                                                      rdfs:label "Method_of_Test_or_Examination" ;
                                                      <http://www.w3.org/2004/02/skos/core#altLabel> "LBMETHOD" ;
                                                      <http://www.w3.org/2004/02/skos/core#definition> "Method of the test or examination. Examples: EIA (Enzyme Immunoassay), ELECTROPHORESIS, DIPSTICK" ;
                                                      <http://www.w3.org/2004/02/skos/core#exactMatch> "Thesaurus:C83312 (http://ncicb.nci.nih.gov/xml/owl/EVS/Thesaurus.owl#C83312)" .


###  https://purls.helmholtz-metadaten.de/ptroDKFZ000070
<https://purls.helmholtz-metadaten.de/ptroDKFZ000070> rdf:type owl:DatatypeProperty ;
                                                      rdfs:domain <http://ncicb.nci.nih.gov/xml/owl/EVS/Thesaurus.owl#C69256> ;
                                                      rdfs:range xsd:string ;
                                                      <http://purl.org/dc/elements/1.1/creator> "OGiraldo" ;
                                                      rdfs:isDefinedBy "https://library.cdisc.org/browser" ;
                                                      rdfs:label "Baseline_Flag" ;
                                                      <http://www.w3.org/2004/02/skos/core#altLabel> "LBBLFL" ;
                                                      <http://www.w3.org/2004/02/skos/core#definition> "A baseline indicator may be used to calculate differences or changes from baseline. Value should be Y or null. The baseline flag is sponsor defined." ;
                                                      <http://www.w3.org/2004/02/skos/core#exactMatch> "Thesaurus:C83303 (http://ncicb.nci.nih.gov/xml/owl/EVS/Thesaurus.owl#C83303)" .


###  https://purls.helmholtz-metadaten.de/ptroDKFZ000071
<https://purls.helmholtz-metadaten.de/ptroDKFZ000071> rdf:type owl:DatatypeProperty ;
                                                      rdfs:domain <http://ncicb.nci.nih.gov/xml/owl/EVS/Thesaurus.owl#C69256> ;
                                                      <http://purl.org/dc/elements/1.1/creator> "OGiraldo" ;
                                                      rdfs:isDefinedBy "https://library.cdisc.org/browser" ;
                                                      rdfs:label "Study_Day_of_Specimen_Collection" ;
                                                      <http://www.w3.org/2004/02/skos/core#altLabel> "LBDY" ;
                                                      <http://www.w3.org/2004/02/skos/core#definition> "Study day of specimen collection, in integer days. The algorithm for calculations must be relative to the sponsor-defined RFSTDTC variable in the Demographics (DM) domain." ;
                                                      <http://www.w3.org/2004/02/skos/core#exactMatch> "Thesaurus:C83306 (http://ncicb.nci.nih.gov/xml/owl/EVS/Thesaurus.owl#C83306)" .


###  https://purls.helmholtz-metadaten.de/ptroDKFZ000072
<https://purls.helmholtz-metadaten.de/ptroDKFZ000072> rdf:type owl:DatatypeProperty ;
                                                      rdfs:domain <http://ncicb.nci.nih.gov/xml/owl/EVS/Thesaurus.owl#C69256> ;
                                                      <http://purl.org/dc/elements/1.1/creator> "OGiraldo" ;
                                                      rdfs:isDefinedBy "https://library.cdisc.org/browser" ;
                                                      rdfs:label "Study_Day_of_End_of_Specimen_Collection" ;
                                                      <http://www.w3.org/2004/02/skos/core#altLabel> "LBENDY" ;
                                                      <http://www.w3.org/2004/02/skos/core#definition> "Study day of the end of specimen collection, in integer days. The algorithm for calculations must be relative to the sponsor-defined RFSTDTC variable in the Demographics (DM) domain." ;
                                                      <http://www.w3.org/2004/02/skos/core#exactMatch> "Thesaurus:C119846 (http://ncicb.nci.nih.gov/xml/owl/EVS/Thesaurus.owl#C119846)" .


###  https://purls.helmholtz-metadaten.de/ptroDKFZ000073
<https://purls.helmholtz-metadaten.de/ptroDKFZ000073> rdf:type owl:DatatypeProperty ;
                                                      rdfs:domain <http://ncicb.nci.nih.gov/xml/owl/EVS/Thesaurus.owl#C69256> ;
                                                      <http://purl.org/dc/elements/1.1/creator> "OGiraldo" ;
                                                      rdfs:isDefinedBy "https://library.cdisc.org/browser" ;
                                                      rdfs:label "Nominal_Study_Day_for_Tabulations" ;
                                                      <http://www.w3.org/2004/02/skos/core#altLabel> "LBNOMDY" ;
                                                      <http://www.w3.org/2004/02/skos/core#definition> "Nominal study day used for grouping records for specimen collections that may occur on different days into a single reported study day. Should be an integer." ;
                                                      <http://www.w3.org/2004/02/skos/core#exactMatch> "Thesaurus:C170498 (http://ncicb.nci.nih.gov/xml/owl/EVS/Thesaurus.owl#C170498)" .


###  https://purls.helmholtz-metadaten.de/ptroDKFZ000074
<https://purls.helmholtz-metadaten.de/ptroDKFZ000074> rdf:type owl:DatatypeProperty ;
                                                      rdfs:domain <http://ncicb.nci.nih.gov/xml/owl/EVS/Thesaurus.owl#C69256> ;
                                                      rdfs:range xsd:string ;
                                                      <http://purl.org/dc/elements/1.1/creator> "OGiraldo" ;
                                                      rdfs:isDefinedBy "https://library.cdisc.org/browser" ;
                                                      rdfs:label "Laboratory_Label_for_Nominal_Study_Day" ;
                                                      <http://www.w3.org/2004/02/skos/core#altLabel> "LBNOMLBL" ;
                                                      <http://www.w3.org/2004/02/skos/core#definition> "A label for a given value of LBNOMDY as presented in the study report. Examples: Week 4, Day 28, Terminal Sac." ;
                                                      <http://www.w3.org/2004/02/skos/core#exactMatch> "Thesaurus:C170499 (http://ncicb.nci.nih.gov/xml/owl/EVS/Thesaurus.owl#C170499)" .


###  https://purls.helmholtz-metadaten.de/ptroDKFZ000083
<https://purls.helmholtz-metadaten.de/ptroDKFZ000083> rdf:type owl:DatatypeProperty ;
                                                      rdfs:domain <http://ncicb.nci.nih.gov/xml/owl/EVS/Thesaurus.owl#C69256> ;
                                                      rdfs:range xsd:string ;
                                                      <http://purl.org/dc/elements/1.1/creator> "OGiraldo" ;
                                                      rdfs:label "Body_Weight_Label_for_Nominal_Study_Day" ;
                                                      <http://www.w3.org/2004/02/skos/core#altLabel> "BWNOMLBL" ;
                                                      <http://www.w3.org/2004/02/skos/core#definition> "A label for a given value of BWNOMDY as presented in the study report. Examples: \"Week 4,\" \"Day 28,\" \"Terminal Sac\"." ;
                                                      <http://www.w3.org/2004/02/skos/core#exactMatch> "Thesaurus:C170499 (http://ncicb.nci.nih.gov/xml/owl/EVS/Thesaurus.owl#C170499)" .


###  https://purls.helmholtz-metadaten.de/ptroDKFZ000090
<https://purls.helmholtz-metadaten.de/ptroDKFZ000090> rdf:type owl:DatatypeProperty ;
                                                      rdfs:domain <http://ncicb.nci.nih.gov/xml/owl/EVS/Thesaurus.owl#C69256> ;
                                                      rdfs:range xsd:string ;
                                                      <http://purl.org/dc/elements/1.1/creator> "OGiraldo" ;
                                                      rdfs:isDefinedBy "https://library.cdisc.org/browser" ;
                                                      rdfs:label "Reported_Name_of_Procedure" ;
                                                      <http://www.w3.org/2004/02/skos/core#altLabel> "PRTRT" ;
                                                      <http://www.w3.org/2004/02/skos/core#definition> "Name of procedure performed, either preprinted or collected on a CRF." ;
                                                      <http://www.w3.org/2004/02/skos/core#exactMatch> "Thesaurus:C117511 (http://ncicb.nci.nih.gov/xml/owl/EVS/Thesaurus.owl#C117511)" .


###  https://purls.helmholtz-metadaten.de/ptroDKFZ000091
<https://purls.helmholtz-metadaten.de/ptroDKFZ000091> rdf:type owl:DatatypeProperty ;
                                                      rdfs:domain <http://ncicb.nci.nih.gov/xml/owl/EVS/Thesaurus.owl#C69256> ;
                                                      rdfs:range xsd:string ;
                                                      <http://purl.org/dc/elements/1.1/creator> "OGiraldo" ;
                                                      rdfs:isDefinedBy "https://library.cdisc.org/browser" ;
                                                      rdfs:label "Identifying_Variable" ;
                                                      <http://www.w3.org/2004/02/skos/core#altLabel> "IDVAR" ;
                                                      <http://www.w3.org/2004/02/skos/core#definition> "Variable in the parent dataset that identifies the record(s) to which the comment applies, which is contained in IDVAR. Examples: BWSEQ or CLGRPID. Used only when individual comments are related to domain records." ;
                                                      <http://www.w3.org/2004/02/skos/core#exactMatch> "Thesaurus:C83293 (http://ncicb.nci.nih.gov/xml/owl/EVS/Thesaurus.owl#C83293)" .


###  https://purls.helmholtz-metadaten.de/ptroDKFZ000092
<https://purls.helmholtz-metadaten.de/ptroDKFZ000092> rdf:type owl:DatatypeProperty ;
                                                      rdfs:domain <http://ncicb.nci.nih.gov/xml/owl/EVS/Thesaurus.owl#C69256> ;
                                                      rdfs:range xsd:string ;
                                                      <http://purl.org/dc/elements/1.1/creator> "OGiraldo" ;
                                                      rdfs:isDefinedBy "https://library.cdisc.org/browser" ;
                                                      rdfs:label "Identifying_Variable_Value" ;
                                                      <http://www.w3.org/2004/02/skos/core#altLabel> "IDVARVAL" ;
                                                      <http://www.w3.org/2004/02/skos/core#definition> "Value of identifying variable of the parent record(s). Used only when individual comments are related to domain records. Cannot be populated if IDVAR is null." ;
                                                      <http://www.w3.org/2004/02/skos/core#exactMatch> "Thesaurus:C83294 (http://ncicb.nci.nih.gov/xml/owl/EVS/Thesaurus.owl#C83294)" .


###  https://purls.helmholtz-metadaten.de/ptroDKFZ000093
<https://purls.helmholtz-metadaten.de/ptroDKFZ000093> rdf:type owl:DatatypeProperty ;
                                                      rdfs:domain <http://ncicb.nci.nih.gov/xml/owl/EVS/Thesaurus.owl#C69256> ;
                                                      rdfs:range xsd:string ;
                                                      <http://purl.org/dc/elements/1.1/creator> "OGiraldo" ;
                                                      rdfs:isDefinedBy "https://library.cdisc.org/browser" ;
                                                      rdfs:label "Comment" ;
                                                      <http://www.w3.org/2004/02/skos/core#altLabel> "COVAL" ;
                                                      <http://www.w3.org/2004/02/skos/core#definition> "The text of the comment. Text over 200 characters can be added to additional columns COVAL1-COVALn. See Assumption 4 in Section 5.2.1.1." ;
                                                      <http://www.w3.org/2004/02/skos/core#exactMatch> "Thesaurus:C83241 (http://ncicb.nci.nih.gov/xml/owl/EVS/Thesaurus.owl#C83241)" .


###  https://purls.helmholtz-metadaten.de/ptroDKFZ000094
<https://purls.helmholtz-metadaten.de/ptroDKFZ000094> rdf:type owl:DatatypeProperty ;
                                                      rdfs:domain <http://ncicb.nci.nih.gov/xml/owl/EVS/Thesaurus.owl#C69256> ;
                                                      rdfs:range xsd:string ;
                                                      <http://purl.org/dc/elements/1.1/creator> "OGiraldo" ;
                                                      rdfs:isDefinedBy "https://library.cdisc.org/browser" ;
                                                      rdfs:label "Comment_Evaluator" ;
                                                      <http://www.w3.org/2004/02/skos/core#altLabel> "COEVAL" ;
                                                      <http://www.w3.org/2004/02/skos/core#definition> "Used to describe the originator of the comment. Examples: TECHNICIAN, STUDY DIRECTOR, VET." ;
                                                      <http://www.w3.org/2004/02/skos/core#exactMatch> "Thesaurus:C83239 (http://ncicb.nci.nih.gov/xml/owl/EVS/Thesaurus.owl#C83239)" .


###  https://purls.helmholtz-metadaten.de/ptroDKFZ000095
<https://purls.helmholtz-metadaten.de/ptroDKFZ000095> rdf:type owl:DatatypeProperty ;
                                                      rdfs:domain <http://ncicb.nci.nih.gov/xml/owl/EVS/Thesaurus.owl#C69256> ;
                                                      rdfs:range xsd:dateTime ;
                                                      <http://purl.org/dc/elements/1.1/creator> "OGiraldo" ;
                                                      rdfs:isDefinedBy "https://library.cdisc.org/browser" ;
                                                      rdfs:label "Date/Time_of_Comment" ;
                                                      <http://www.w3.org/2004/02/skos/core#altLabel> "CODTC" ;
                                                      <http://www.w3.org/2004/02/skos/core#definition> "Date/Time of the comment, in ISO 8601 format. May be null if this is a child record of another domain or if the comment date was not collected. In all other cases, this represents the date/time of the comment in ISO 8601 format." ;
                                                      <http://www.w3.org/2004/02/skos/core#exactMatch> "Thesaurus:C83238 (http://ncicb.nci.nih.gov/xml/owl/EVS/Thesaurus.owl#C83238)" .


###  https://purls.helmholtz-metadaten.de/ptroDKFZ000096
<https://purls.helmholtz-metadaten.de/ptroDKFZ000096> rdf:type owl:DatatypeProperty ;
                                                      rdfs:domain <http://ncicb.nci.nih.gov/xml/owl/EVS/Thesaurus.owl#C69256> ;
                                                      rdfs:range xsd:decimal ;
                                                      <http://purl.org/dc/elements/1.1/creator> "OGiraldo" ;
                                                      rdfs:isDefinedBy "https://library.cdisc.org/browser" ;
                                                      rdfs:label "Study_Day_of_Comment" ;
                                                      <http://www.w3.org/2004/02/skos/core#altLabel> "CODY" ;
                                                      <http://www.w3.org/2004/02/skos/core#definition> "Study day of the comment, in integer days. May be null if this is a child record of another domain or if the comment date was not collected. The algorithm for calculations must be relative to the sponsor-defined RFSTDTC variable in the Demographics (DM) domain." ;
                                                      <http://www.w3.org/2004/02/skos/core#exactMatch> "Thesaurus:C119819 (http://ncicb.nci.nih.gov/xml/owl/EVS/Thesaurus.owl#C119819)" .


###  https://purls.helmholtz-metadaten.de/ptroDKFZ000097
<https://purls.helmholtz-metadaten.de/ptroDKFZ000097> rdf:type owl:DatatypeProperty ;
                                                      rdfs:domain <http://ncicb.nci.nih.gov/xml/owl/EVS/Thesaurus.owl#C69256> ;
                                                      rdfs:range xsd:string ;
                                                      <http://purl.org/dc/elements/1.1/creator> "OGiraldo" ;
                                                      rdfs:isDefinedBy "https://library.cdisc.org/browser" ;
                                                      rdfs:label "Standardized_Procedure_Name" ;
                                                      <http://www.w3.org/2004/02/skos/core#altLabel> "PRDECOD" ;
                                                      <http://www.w3.org/2004/02/skos/core#definition> "Standardized or dictionary-derived name of PRTRT. If the codelist \"PROCEDUR\" is not used, the sponsor is expected to provide the dictionary name and version used to map the terms in the external codelist element in the Define-XML document. If an intervention term does not have a decode value, then PRDECOD will be null." ;
                                                      <http://www.w3.org/2004/02/skos/core#exactMatch> "Thesaurus:C117512 (http://ncicb.nci.nih.gov/xml/owl/EVS/Thesaurus.owl#C117512)" .


###  https://purls.helmholtz-metadaten.de/ptroDKFZ000098
<https://purls.helmholtz-metadaten.de/ptroDKFZ000098> rdf:type owl:DatatypeProperty ;
                                                      rdfs:domain <http://ncicb.nci.nih.gov/xml/owl/EVS/Thesaurus.owl#C69256> ;
                                                      rdfs:range xsd:string ;
                                                      <http://purl.org/dc/elements/1.1/creator> "OGiraldo" ;
                                                      rdfs:isDefinedBy "https://library.cdisc.org/browser" ;
                                                      rdfs:label "Procedure_Category" ;
                                                      <http://www.w3.org/2004/02/skos/core#altLabel> "PRCAT" ;
                                                      <http://www.w3.org/2004/02/skos/core#definition> "Used to define a category of procedure values." ;
                                                      <http://www.w3.org/2004/02/skos/core#exactMatch> "Thesaurus:C117513 (http://ncicb.nci.nih.gov/xml/owl/EVS/Thesaurus.owl#C117513)" .


###  https://purls.helmholtz-metadaten.de/ptroDKFZ000099
<https://purls.helmholtz-metadaten.de/ptroDKFZ000099> rdf:type owl:DatatypeProperty ;
                                                      rdfs:domain <http://ncicb.nci.nih.gov/xml/owl/EVS/Thesaurus.owl#C69256> ;
                                                      rdfs:range xsd:string ;
                                                      <http://purl.org/dc/elements/1.1/creator> "OGiraldo" ;
                                                      rdfs:isDefinedBy "https://library.cdisc.org/browser" ;
                                                      rdfs:label "Procedure_Subcategory" ;
                                                      <http://www.w3.org/2004/02/skos/core#altLabel> "PRSCAT" ;
                                                      <http://www.w3.org/2004/02/skos/core#definition> "Used to define a further categorization of PRCAT values." ;
                                                      <http://www.w3.org/2004/02/skos/core#exactMatch> "Thesaurus:C117514 (http://ncicb.nci.nih.gov/xml/owl/EVS/Thesaurus.owl#C117514)" .


###  https://purls.helmholtz-metadaten.de/ptroDKFZ000100
<https://purls.helmholtz-metadaten.de/ptroDKFZ000100> rdf:type owl:DatatypeProperty ;
                                                      rdfs:domain <http://ncicb.nci.nih.gov/xml/owl/EVS/Thesaurus.owl#C69256> ;
                                                      rdfs:range xsd:string ;
                                                      <http://purl.org/dc/elements/1.1/creator> "OGiraldo" ;
                                                      rdfs:isDefinedBy "https://library.cdisc.org/browser" ;
                                                      rdfs:label "Procedure_Prespecified" ;
                                                      <http://www.w3.org/2004/02/skos/core#altLabel> "PRPRESP" ;
                                                      <http://www.w3.org/2004/02/skos/core#definition> "Used when a specific procedure is pre-specified on a CRF. Values should be \"Y\" or null." ;
                                                      <http://www.w3.org/2004/02/skos/core#exactMatch> "Thesaurus:C117528 (http://ncicb.nci.nih.gov/xml/owl/EVS/Thesaurus.owl#C117528)" .


###  https://purls.helmholtz-metadaten.de/ptroDKFZ000101
<https://purls.helmholtz-metadaten.de/ptroDKFZ000101> rdf:type owl:DatatypeProperty ;
                                                      rdfs:domain <http://ncicb.nci.nih.gov/xml/owl/EVS/Thesaurus.owl#C69256> ;
                                                      rdfs:range xsd:string ;
                                                      <http://purl.org/dc/elements/1.1/creator> "OGiraldo" ;
                                                      rdfs:isDefinedBy "https://library.cdisc.org/browser" ;
                                                      rdfs:label "Procedure_Occurrence" ;
                                                      <http://www.w3.org/2004/02/skos/core#altLabel> "PROCCUR" ;
                                                      <http://www.w3.org/2004/02/skos/core#definition> "Used to record whether a prespecified procedure occurred when information about the occurrence of a specific procedure is solicited." ;
                                                      <http://www.w3.org/2004/02/skos/core#exactMatch> "Thesaurus:C117516 (http://ncicb.nci.nih.gov/xml/owl/EVS/Thesaurus.owl#C117516)" .


###  https://purls.helmholtz-metadaten.de/ptroDKFZ000102
<https://purls.helmholtz-metadaten.de/ptroDKFZ000102> rdf:type owl:DatatypeProperty ;
                                                      rdfs:domain <http://ncicb.nci.nih.gov/xml/owl/EVS/Thesaurus.owl#C69256> ;
                                                      rdfs:range xsd:decimal ;
                                                      <http://purl.org/dc/elements/1.1/creator> "OGiraldo" ;
                                                      rdfs:isDefinedBy "https://library.cdisc.org/browser" ;
                                                      rdfs:label "Procedure_Dose" ;
                                                      <http://www.w3.org/2004/02/skos/core#altLabel> "PRDOSE" ;
                                                      <http://www.w3.org/2004/02/skos/core#definition> "Amount of PRTRT administered. Not populated when PRDOSTXT is populated." ;
                                                      <http://www.w3.org/2004/02/skos/core#exactMatch> "Thesaurus:C117518 (http://ncicb.nci.nih.gov/xml/owl/EVS/Thesaurus.owl#C117518)" .


###  https://purls.helmholtz-metadaten.de/ptroDKFZ000103
<https://purls.helmholtz-metadaten.de/ptroDKFZ000103> rdf:type owl:DatatypeProperty ;
                                                      rdfs:domain <http://ncicb.nci.nih.gov/xml/owl/EVS/Thesaurus.owl#C69256> ;
                                                      rdfs:range xsd:string ;
                                                      <http://purl.org/dc/elements/1.1/creator> "OGiraldo" ;
                                                      rdfs:isDefinedBy "https://library.cdisc.org/browser" ;
                                                      rdfs:label "Procedure_Dose_Units" ;
                                                      <http://www.w3.org/2004/02/skos/core#altLabel> "PRDOSU" ;
                                                      <http://www.w3.org/2004/02/skos/core#definition> "Units for PRDOSE, PRDOSTOT, or PRDOSTXT." ;
                                                      <http://www.w3.org/2004/02/skos/core#exactMatch> "Thesaurus:C117520 (http://ncicb.nci.nih.gov/xml/owl/EVS/Thesaurus.owl#C117520)" .


###  https://purls.helmholtz-metadaten.de/ptroDKFZ000104
<https://purls.helmholtz-metadaten.de/ptroDKFZ000104> rdf:type owl:DatatypeProperty ;
                                                      rdfs:domain <http://ncicb.nci.nih.gov/xml/owl/EVS/Thesaurus.owl#C69256> ;
                                                      rdfs:range xsd:string ;
                                                      <http://purl.org/dc/elements/1.1/creator> "OGiraldo" ;
                                                      rdfs:isDefinedBy "https://library.cdisc.org/browser" ;
                                                      rdfs:label "Procedure_Dosing_Frequency_per_Interval" ;
                                                      <http://www.w3.org/2004/02/skos/core#altLabel> "PRDOSFRQ" ;
                                                      <http://www.w3.org/2004/02/skos/core#definition> "Usually expressed as the number of doses given per a specific interval." ;
                                                      <http://www.w3.org/2004/02/skos/core#exactMatch> "Thesaurus:C117522 (http://ncicb.nci.nih.gov/xml/owl/EVS/Thesaurus.owl#C117522)" .


###  https://purls.helmholtz-metadaten.de/ptroDKFZ000105
<https://purls.helmholtz-metadaten.de/ptroDKFZ000105> rdf:type owl:DatatypeProperty ;
                                                      rdfs:domain <http://ncicb.nci.nih.gov/xml/owl/EVS/Thesaurus.owl#C69256> ;
                                                      rdfs:range xsd:string ;
                                                      <http://purl.org/dc/elements/1.1/creator> "OGiraldo" ;
                                                      rdfs:isDefinedBy "https://library.cdisc.org/browser" ;
                                                      rdfs:label "Location_of_Procedure" ;
                                                      <http://www.w3.org/2004/02/skos/core#altLabel> "PRLOC" ;
                                                      <http://www.w3.org/2004/02/skos/core#definition> "Anatomical location of a procedure." ;
                                                      <http://www.w3.org/2004/02/skos/core#exactMatch> "Thesaurus:C117525 (http://ncicb.nci.nih.gov/xml/owl/EVS/Thesaurus.owl#C117525)" .


###  https://purls.helmholtz-metadaten.de/ptroDKFZ000106
<https://purls.helmholtz-metadaten.de/ptroDKFZ000106> rdf:type owl:DatatypeProperty ;
                                                      rdfs:domain <http://ncicb.nci.nih.gov/xml/owl/EVS/Thesaurus.owl#C69256> ;
                                                      rdfs:range xsd:string ;
                                                      <http://purl.org/dc/elements/1.1/creator> "OGiraldo" ;
                                                      rdfs:isDefinedBy "https://library.cdisc.org/browser" ;
                                                      rdfs:label "Procedure_Laterality" ;
                                                      <http://www.w3.org/2004/02/skos/core#altLabel> "PRLAT" ;
                                                      <http://www.w3.org/2004/02/skos/core#definition> "Qualifier for anatomical location or specimen further detailing laterality." ;
                                                      <http://www.w3.org/2004/02/skos/core#exactMatch> "Thesaurus:C117526 (http://ncicb.nci.nih.gov/xml/owl/EVS/Thesaurus.owl#C117526)" .


###  https://purls.helmholtz-metadaten.de/ptroDKFZ000107
<https://purls.helmholtz-metadaten.de/ptroDKFZ000107> rdf:type owl:DatatypeProperty ;
                                                      rdfs:domain <http://ncicb.nci.nih.gov/xml/owl/EVS/Thesaurus.owl#C69256> ;
                                                      rdfs:range xsd:string ;
                                                      <http://purl.org/dc/elements/1.1/creator> "OGiraldo" ;
                                                      rdfs:isDefinedBy "https://library.cdisc.org/browser" ;
                                                      rdfs:label "Procedure_Directionality" ;
                                                      <http://www.w3.org/2004/02/skos/core#altLabel> "PRDIR" ;
                                                      <http://www.w3.org/2004/02/skos/core#definition> "Qualifier for anatomical location or specimen further detailing directionality." ;
                                                      <http://www.w3.org/2004/02/skos/core#exactMatch> "Thesaurus:C117527 (http://ncicb.nci.nih.gov/xml/owl/EVS/Thesaurus.owl#C117527)" .


###  https://purls.helmholtz-metadaten.de/ptroDKFZ000108
<https://purls.helmholtz-metadaten.de/ptroDKFZ000108> rdf:type owl:DatatypeProperty ;
                                                      rdfs:domain <http://ncicb.nci.nih.gov/xml/owl/EVS/Thesaurus.owl#C69256> ;
                                                      rdfs:range xsd:string ;
                                                      <http://purl.org/dc/elements/1.1/creator> "OGiraldo" ;
                                                      rdfs:isDefinedBy "https://library.cdisc.org/browser" ;
                                                      rdfs:label "Procedure_Portion_or_Totality" ;
                                                      <http://www.w3.org/2004/02/skos/core#altLabel> "PRPORTOT" ;
                                                      <http://www.w3.org/2004/02/skos/core#definition> "Qualifier for anatomical location or specimen further detailing the distribution, which means arrangement of, apportioning of." ;
                                                      <http://www.w3.org/2004/02/skos/core#exactMatch> "Thesaurus:C117528 (http://ncicb.nci.nih.gov/xml/owl/EVS/Thesaurus.owl#C117528)" .


###  https://purls.helmholtz-metadaten.de/ptroDKFZ000109
<https://purls.helmholtz-metadaten.de/ptroDKFZ000109> rdf:type owl:DatatypeProperty ;
                                                      rdfs:domain <http://ncicb.nci.nih.gov/xml/owl/EVS/Thesaurus.owl#C69256> ;
                                                      rdfs:range xsd:dateTime ;
                                                      <http://purl.org/dc/elements/1.1/creator> "OGiraldo" ;
                                                      rdfs:isDefinedBy "https://library.cdisc.org/browser" ;
                                                      rdfs:label "Start_Date/Time_of_Procedure" ;
                                                      <http://www.w3.org/2004/02/skos/core#altLabel> "PRSTDTC" ;
                                                      <http://www.w3.org/2004/02/skos/core#definition> "Start date/time of the procedure represented in ISO 8601 character format." ;
                                                      <http://www.w3.org/2004/02/skos/core#exactMatch> "Thesaurus:C117529 (http://ncicb.nci.nih.gov/xml/owl/EVS/Thesaurus.owl#C117529)" .


###  https://purls.helmholtz-metadaten.de/ptroDKFZ000110
<https://purls.helmholtz-metadaten.de/ptroDKFZ000110> rdf:type owl:DatatypeProperty ;
                                                      rdfs:domain <http://ncicb.nci.nih.gov/xml/owl/EVS/Thesaurus.owl#C69256> ;
                                                      rdfs:range xsd:dateTime ;
                                                      <http://purl.org/dc/elements/1.1/creator> "OGiraldo" ;
                                                      rdfs:isDefinedBy "https://library.cdisc.org/browser" ;
                                                      rdfs:label "End_Date/Time_of_Procedure" ;
                                                      <http://www.w3.org/2004/02/skos/core#altLabel> "PRENDTC" ;
                                                      <http://www.w3.org/2004/02/skos/core#definition> "End date/time of the procedure represented in ISO 8601 character format." ;
                                                      <http://www.w3.org/2004/02/skos/core#exactMatch> "Thesaurus:C117530 (http://ncicb.nci.nih.gov/xml/owl/EVS/Thesaurus.owl#C117530)" .


###  https://purls.helmholtz-metadaten.de/ptroDKFZ000111
<https://purls.helmholtz-metadaten.de/ptroDKFZ000111> rdf:type owl:DatatypeProperty ;
                                                      rdfs:domain <http://ncicb.nci.nih.gov/xml/owl/EVS/Thesaurus.owl#C69256> ;
                                                      rdfs:range xsd:decimal ;
                                                      <http://purl.org/dc/elements/1.1/creator> "OGiraldo" ;
                                                      rdfs:isDefinedBy "https://library.cdisc.org/browser" ;
                                                      rdfs:label "Study_Day_of_Start_of_Procedure" ;
                                                      <http://www.w3.org/2004/02/skos/core#altLabel> "PRSTDY" ;
                                                      <http://www.w3.org/2004/02/skos/core#definition> "Study day of start of procedure expressed in integer days relative to the sponsor-defined RFSTDTC in Demographics." ;
                                                      <http://www.w3.org/2004/02/skos/core#exactMatch> "Thesaurus:C117531 (http://ncicb.nci.nih.gov/xml/owl/EVS/Thesaurus.owl#C117531)" .


###  https://purls.helmholtz-metadaten.de/ptroDKFZ000112
<https://purls.helmholtz-metadaten.de/ptroDKFZ000112> rdf:type owl:DatatypeProperty ;
                                                      rdfs:domain <http://ncicb.nci.nih.gov/xml/owl/EVS/Thesaurus.owl#C69256> ;
                                                      rdfs:range xsd:decimal ;
                                                      <http://purl.org/dc/elements/1.1/creator> "OGiraldo" ;
                                                      rdfs:isDefinedBy "https://library.cdisc.org/browser" ;
                                                      rdfs:label "Study_Day_of_End_of_Procedure" ;
                                                      <http://www.w3.org/2004/02/skos/core#altLabel> "PRENDY" ;
                                                      <http://www.w3.org/2004/02/skos/core#definition> "Study day of end of procedure expressed in integer days relative to the sponsor-defined RFSTDTC in Demographics." ;
                                                      <http://www.w3.org/2004/02/skos/core#exactMatch> "Thesaurus:C117532 (http://ncicb.nci.nih.gov/xml/owl/EVS/Thesaurus.owl#C117532)" .


###  https://purls.helmholtz-metadaten.de/ptroDKFZ000113
<https://purls.helmholtz-metadaten.de/ptroDKFZ000113> rdf:type owl:DatatypeProperty ;
                                                      rdfs:domain <http://ncicb.nci.nih.gov/xml/owl/EVS/Thesaurus.owl#C69256> ;
                                                      rdfs:range xsd:string ;
                                                      <http://purl.org/dc/elements/1.1/creator> "OGiraldo" ;
                                                      rdfs:isDefinedBy "https://library.cdisc.org/browser" ;
                                                      rdfs:label "Duration_of_Procedure" ;
                                                      <http://www.w3.org/2004/02/skos/core#altLabel> "PRDUR" ;
                                                      <http://www.w3.org/2004/02/skos/core#definition> "Collected duration of a procedure represented in ISO 8601 character format. Used only if collected on the CRF and not derived from start and end date/times." ;
                                                      <http://www.w3.org/2004/02/skos/core#exactMatch> "Thesaurus:C117533 (http://ncicb.nci.nih.gov/xml/owl/EVS/Thesaurus.owl#C117533)" .


###  https://purls.helmholtz-metadaten.de/ptroDKFZ000115
<https://purls.helmholtz-metadaten.de/ptroDKFZ000115> rdf:type owl:DatatypeProperty ;
                                                      rdfs:domain <http://ncicb.nci.nih.gov/xml/owl/EVS/Thesaurus.owl#C69256> ;
                                                      rdfs:range xsd:string ;
                                                      rdfs:comment "This attribute is not part of the CDISC standard; it was defined by our DKFZ working group (E220)." ;
                                                      rdfs:isDefinedBy "E220" ;
                                                      rdfs:label "Project_Unique_Identifier" ;
                                                      <http://www.w3.org/2004/02/skos/core#altLabel> "PUID" ;
                                                      <http://www.w3.org/2004/02/skos/core#definition> "A unique alphanumeric identifier assigned to a project to ensure its distinct identification within a given system, organization, or dataset." .


###  https://purls.helmholtz-metadaten.de/ptroDKFZ000116
<https://purls.helmholtz-metadaten.de/ptroDKFZ000116> rdf:type owl:DatatypeProperty ;
                                                      rdfs:domain <http://ncicb.nci.nih.gov/xml/owl/EVS/Thesaurus.owl#C69256> ;
                                                      rdfs:range xsd:string ;
                                                      <http://purl.org/dc/elements/1.1/creator> "OGiraldo" ;
                                                      rdfs:isDefinedBy "https://library.cdisc.org/browser" ;
                                                      rdfs:label "Planned_Arm_Code" ;
                                                      <http://www.w3.org/2004/02/skos/core#altLabel> "ARMCD" ;
                                                      <http://www.w3.org/2004/02/skos/core#definition> "Short name for ARM (may be up to 20 characters) used for sorting and programming. Should be populated when Arms have been defined in the TA domain." ;
                                                      <http://www.w3.org/2004/02/skos/core#exactMatch> "Thesaurus:C83216 (http://ncicb.nci.nih.gov/xml/owl/EVS/Thesaurus.owl#C83216)" .


###  https://purls.helmholtz-metadaten.de/ptroDKFZ000117
<https://purls.helmholtz-metadaten.de/ptroDKFZ000117> rdf:type owl:DatatypeProperty ;
                                                      rdfs:domain <http://ncicb.nci.nih.gov/xml/owl/EVS/Thesaurus.owl#C69256> ;
                                                      rdfs:range xsd:string ;
                                                      <http://purl.org/dc/elements/1.1/creator> "OGiraldo" ;
                                                      rdfs:isDefinedBy "https://library.cdisc.org/browser" ;
                                                      rdfs:label "Description_of_Planned_Arm" ;
                                                      <http://www.w3.org/2004/02/skos/core#altLabel> "ARM" ;
                                                      <http://www.w3.org/2004/02/skos/core#definition> "Descriptive name given to a specific Trial Arm (e.g., Low Dose, Mid Dose, 10 mg/kg/day dose, Third Arm) to which the subject was assigned." .


###  https://purls.helmholtz-metadaten.de/ptroDKFZ000118
<https://purls.helmholtz-metadaten.de/ptroDKFZ000118> rdf:type owl:DatatypeProperty ;
                                                      rdfs:domain <http://ncicb.nci.nih.gov/xml/owl/EVS/Thesaurus.owl#C69256> ;
                                                      rdfs:range xsd:string ;
                                                      <http://purl.org/dc/elements/1.1/creator> "OGiraldo" ;
                                                      rdfs:isDefinedBy "https://library.cdisc.org/browser" ;
                                                      rdfs:label "Set_Code" ;
                                                      <http://www.w3.org/2004/02/skos/core#altLabel> "SETCD" ;
                                                      <http://www.w3.org/2004/02/skos/core#definition> "Short name of a specific Trial Set to which the subject was assigned, as defined by the sponsor. Maximum of 8 characters. This represents the Trial Set for which parameters are being submitted." ;
                                                      <http://www.w3.org/2004/02/skos/core#exactMatch> "Thesaurus:C117457 (http://ncicb.nci.nih.gov/xml/owl/EVS/Thesaurus.owl#C117457)" .


#################################################################
#    Classes
#################################################################

###  http://ncicb.nci.nih.gov/xml/owl/EVS/Thesaurus.owl#C14238
<http://ncicb.nci.nih.gov/xml/owl/EVS/Thesaurus.owl#C14238> rdf:type owl:Class ;
                                                            rdfs:subClassOf <http://purl.bioontology.org/ontology/STY/T015> ;
                                                            <http://purl.org/dc/elements/1.1/creator> "OGiraldo" ;
                                                            rdfs:isDefinedBy "http://purl.bioontology.org/ontology/NCIT" ;
                                                            rdfs:label "Mouse" ;
                                                            <http://www.w3.org/2004/02/skos/core#definition> "Any of numerous species of small rodents belonging to the genus Mus and various related genera of the family Muridae." .


###  http://ncicb.nci.nih.gov/xml/owl/EVS/Thesaurus.owl#C25364
<http://ncicb.nci.nih.gov/xml/owl/EVS/Thesaurus.owl#C25364> rdf:type owl:Class ;
                                                            rdfs:subClassOf <http://purl.bioontology.org/ontology/STY/T170> ;
                                                            rdfs:isDefinedBy "http://purl.bioontology.org/ontology/NCIT" ;
                                                            rdfs:label "Identifier"@en ;
                                                            <http://www.w3.org/2004/02/skos/core#definition> "One or more characters used to identify, name, or characterize the nature, properties, or contents of a thing."@en .


###  http://ncicb.nci.nih.gov/xml/owl/EVS/Thesaurus.owl#C49569
<http://ncicb.nci.nih.gov/xml/owl/EVS/Thesaurus.owl#C49569> rdf:type owl:Class ;
                                                            rdfs:subClassOf <http://ncicb.nci.nih.gov/xml/owl/EVS/Thesaurus.owl#C62289> ;
                                                            <http://purl.org/dc/elements/1.1/creator> "OGiraldo" ;
                                                            rdfs:isDefinedBy "A subject domain utilized for the submission of information encompassing and representing data, vocabulary or records related to comments." ,
                                                                             "http://purl.bioontology.org/ontology/NCIT" ;
                                                            rdfs:label "Comment Domain" ;
                                                            <http://www.w3.org/2004/02/skos/core#altLabel> "CO, Comments" .


###  http://ncicb.nci.nih.gov/xml/owl/EVS/Thesaurus.owl#C49572
<http://ncicb.nci.nih.gov/xml/owl/EVS/Thesaurus.owl#C49572> rdf:type owl:Class ;
                                                            rdfs:subClassOf <http://ncicb.nci.nih.gov/xml/owl/EVS/Thesaurus.owl#C62289> ;
                                                            <http://purl.org/dc/elements/1.1/creator> "OGiraldo" ;
                                                            rdfs:isDefinedBy "http://purl.bioontology.org/ontology/NCIT" ;
                                                            rdfs:label "Demographics Domain" ;
                                                            <http://www.w3.org/2004/02/skos/core#altLabel> "Demographics, DM" ;
                                                            <http://www.w3.org/2004/02/skos/core#definition> "A subject domain utilized for the submission of information encompassing and representing data, vocabulary or records related to comments." .


###  http://ncicb.nci.nih.gov/xml/owl/EVS/Thesaurus.owl#C49587
<http://ncicb.nci.nih.gov/xml/owl/EVS/Thesaurus.owl#C49587> rdf:type owl:Class ;
                                                            rdfs:subClassOf <http://ncicb.nci.nih.gov/xml/owl/EVS/Thesaurus.owl#C62289> ;
                                                            <http://purl.org/dc/elements/1.1/creator> "OGiraldo" ;
                                                            rdfs:isDefinedBy "http://purl.bioontology.org/ontology/NCIT" ;
                                                            rdfs:label "Exposure Domain" ;
                                                            <http://www.w3.org/2004/02/skos/core#altLabel> "EX, Exposure" ;
                                                            <http://www.w3.org/2004/02/skos/core#definition> "A subject domain utilized for the submission of information encompassing and representing data, vocabulary or records related to exposure." .


###  http://ncicb.nci.nih.gov/xml/owl/EVS/Thesaurus.owl#C49592
<http://ncicb.nci.nih.gov/xml/owl/EVS/Thesaurus.owl#C49592> rdf:type owl:Class ;
                                                            rdfs:subClassOf <http://ncicb.nci.nih.gov/xml/owl/EVS/Thesaurus.owl#C62289> ;
                                                            <http://purl.org/dc/elements/1.1/creator> "OGiraldo" ;
                                                            rdfs:isDefinedBy "http://purl.bioontology.org/ontology/NCIT" ;
                                                            rdfs:label "Laboratory Data Domain" ;
                                                            <http://www.w3.org/2004/02/skos/core#altLabel> "Laboratory Test Results, LB" ;
                                                            <http://www.w3.org/2004/02/skos/core#definition> "A subject domain utilized for the submission of information encompassing and representing data, vocabulary or records related to laboratory data." .


###  http://ncicb.nci.nih.gov/xml/owl/EVS/Thesaurus.owl#C54100
<http://ncicb.nci.nih.gov/xml/owl/EVS/Thesaurus.owl#C54100> rdf:type owl:Class ;
                                                            rdfs:subClassOf <http://ncicb.nci.nih.gov/xml/owl/EVS/Thesaurus.owl#C70663> ;
                                                            rdfs:isDefinedBy "http://purl.bioontology.org/ontology/NCIT" ;
                                                            rdfs:label "Universally Unique Identifier"@en ;
                                                            <http://www.w3.org/2004/02/skos/core#definition> "A 128 bit identifier. Depending on the mechanism used to generate it, it is either guaranteed to be different from all other UUIDs/GUIDs generated until 3400 AD or extremely likely to be different. Its relatively small size lends itself well to sorting, ordering, and hashing of all sorts, storing in databases, simple allocation, and ease of programming in general."@en .


###  http://ncicb.nci.nih.gov/xml/owl/EVS/Thesaurus.owl#C62289
<http://ncicb.nci.nih.gov/xml/owl/EVS/Thesaurus.owl#C62289> rdf:type owl:Class ;
                                                            rdfs:subClassOf <http://purl.bioontology.org/ontology/STY/T077> ;
                                                            <http://purl.org/dc/elements/1.1/creator> "OGiraldo" ;
                                                            rdfs:isDefinedBy "http://purl.bioontology.org/ontology/NCIT" ;
                                                            rdfs:label "Domain" ;
                                                            <http://www.w3.org/2004/02/skos/core#definition> "An area of knowledge considered as a discrete unit for some purpose." .


###  http://ncicb.nci.nih.gov/xml/owl/EVS/Thesaurus.owl#C69219
<http://ncicb.nci.nih.gov/xml/owl/EVS/Thesaurus.owl#C69219> rdf:type owl:Class ;
                                                            rdfs:subClassOf <http://ncicb.nci.nih.gov/xml/owl/EVS/Thesaurus.owl#C71160> ;
                                                            rdfs:isDefinedBy "http://purl.bioontology.org/ontology/NCIT" ;
                                                            rdfs:label "Series Instance UID"@en ;
                                                            <http://www.w3.org/2004/02/skos/core#definition> "A unique identifier for series of images."@en .


###  http://ncicb.nci.nih.gov/xml/owl/EVS/Thesaurus.owl#C69256
<http://ncicb.nci.nih.gov/xml/owl/EVS/Thesaurus.owl#C69256> rdf:type owl:Class ;
                                                            rdfs:subClassOf <http://ncicb.nci.nih.gov/xml/owl/EVS/Thesaurus.owl#C70663> ;
                                                            rdfs:comment "aka 'Unique Subject Identifier (USUBJID)' at CDISC; and 'Subject Id' at RPB." ;
                                                            rdfs:isDefinedBy "http://purl.bioontology.org/ontology/NCIT" ;
                                                            rdfs:label "Subject Unique Identifier" ;
                                                            <http://www.w3.org/2004/02/skos/core#definition> "A unique identifier for a subject in a study." .


###  http://ncicb.nci.nih.gov/xml/owl/EVS/Thesaurus.owl#C70663
<http://ncicb.nci.nih.gov/xml/owl/EVS/Thesaurus.owl#C70663> rdf:type owl:Class ;
                                                            rdfs:subClassOf <http://ncicb.nci.nih.gov/xml/owl/EVS/Thesaurus.owl#C25364> ;
                                                            rdfs:isDefinedBy "http://purl.bioontology.org/ontology/NCIT" ;
                                                            rdfs:label "Unique Identifier"@en ;
                                                            <http://www.w3.org/2004/02/skos/core#definition> "A set of characters used as a code that is unique in the context or the system for which it is created. It serves as a means of identification and reference (often instead of a name) for an entity, person, thing, function, procedure, activity, variable, or body of data."@en .


###  http://ncicb.nci.nih.gov/xml/owl/EVS/Thesaurus.owl#C71160
<http://ncicb.nci.nih.gov/xml/owl/EVS/Thesaurus.owl#C71160> rdf:type owl:Class ;
                                                            rdfs:subClassOf <http://ncicb.nci.nih.gov/xml/owl/EVS/Thesaurus.owl#C70663> ;
                                                            rdfs:isDefinedBy "http://purl.bioontology.org/ontology/NCIT" ;
                                                            rdfs:label "Instance Unique Identifier"@en ;
                                                            <http://www.w3.org/2004/02/skos/core#definition> "Data type unique identifier within a particular context."@en .


###  http://ncicb.nci.nih.gov/xml/owl/EVS/Thesaurus.owl#C83083
<http://ncicb.nci.nih.gov/xml/owl/EVS/Thesaurus.owl#C83083> rdf:type owl:Class ;
                                                            owl:equivalentClass <https://purls.helmholtz-metadaten.de/ptroDKFZ000006> ;
                                                            rdfs:subClassOf <http://ncicb.nci.nih.gov/xml/owl/EVS/Thesaurus.owl#C25364> ;
                                                            rdfs:comment "aka 'Subject Identifier for the Study (SUBJID)' at CDICS, and 'subject identification' at RPB." ;
                                                            rdfs:isDefinedBy "http://purl.bioontology.org/ontology/NCIT" ;
                                                            rdfs:label "Subject Identifier" ;
                                                            <http://www.w3.org/2004/02/skos/core#altLabel> "Studynumber" ;
                                                            <http://www.w3.org/2004/02/skos/core#definition> "" ,
                                                                                                             "A sequence of characters used to identify, name, or characterize the study subject." .


###  http://ncicb.nci.nih.gov/xml/owl/EVS/Thesaurus.owl#C95085
<http://ncicb.nci.nih.gov/xml/owl/EVS/Thesaurus.owl#C95085> rdf:type owl:Class ;
                                                            rdfs:subClassOf <http://ncicb.nci.nih.gov/xml/owl/EVS/Thesaurus.owl#C62289> ;
                                                            <http://purl.org/dc/elements/1.1/creator> "OGiraldo" ;
                                                            rdfs:isDefinedBy "http://purl.bioontology.org/ontology/NCIT" ;
                                                            rdfs:label "Body Weight Domain" ;
                                                            <http://www.w3.org/2004/02/skos/core#altLabel> "Body Weight, BW" ;
                                                            <http://www.w3.org/2004/02/skos/core#definition> "A subject domain utilized for the submission of information encompassing and representing data, vocabulary or records related to body weight." .


###  http://ncicb.nci.nih.gov/xml/owl/EVS/Thesaurus.owl#C95086
<http://ncicb.nci.nih.gov/xml/owl/EVS/Thesaurus.owl#C95086> rdf:type owl:Class ;
                                                            rdfs:subClassOf <http://ncicb.nci.nih.gov/xml/owl/EVS/Thesaurus.owl#C62289> ;
                                                            <http://purl.org/dc/elements/1.1/creator> "OGiraldo" ;
                                                            rdfs:isDefinedBy "http://purl.bioontology.org/ontology/NCIT" ;
                                                            rdfs:label "Clinical Observation Domain" ;
                                                            <http://www.w3.org/2004/02/skos/core#altLabel> "Clinical Observation, CL" ;
                                                            <http://www.w3.org/2004/02/skos/core#definition> "A subject domain utilized for the submission of information encompassing and representing data, vocabulary or records related to clinical observations." .


###  http://ncicb.nci.nih.gov/xml/owl/EVS/Thesaurus.owl#C95087
<http://ncicb.nci.nih.gov/xml/owl/EVS/Thesaurus.owl#C95087> rdf:type owl:Class ;
                                                            rdfs:subClassOf <http://ncicb.nci.nih.gov/xml/owl/EVS/Thesaurus.owl#C62289> ;
                                                            <http://purl.org/dc/elements/1.1/creator> "OGiraldo" ;
                                                            rdfs:isDefinedBy "http://purl.bioontology.org/ontology/NCIT" ;
                                                            rdfs:label "Death Diagnosis Domain" ;
                                                            <http://www.w3.org/2004/02/skos/core#altLabel> "Death Diagnosis and Details, Death Details, DD" ;
                                                            <http://www.w3.org/2004/02/skos/core#definition> "A subject domain utilized for the submission of information encompassing and representing data, vocabulary or records related to death diagnosis." .


###  http://purl.bioontology.org/ontology/STY/T001
<http://purl.bioontology.org/ontology/STY/T001> rdf:type owl:Class ;
                                                rdfs:subClassOf <http://purl.bioontology.org/ontology/STY/T072> ;
                                                rdfs:isDefinedBy "http://purl.bioontology.org/ontology/STY" ;
                                                rdfs:label "Organism"@en ;
                                                <http://www.w3.org/2004/02/skos/core#definition> "Generally, a living individual, including all plants and animals."@en ;
                                                <http://www.w3.org/2004/02/skos/core#exactMatch> "Thesaurus:C14250 (http://ncicb.nci.nih.gov/xml/owl/EVS/Thesaurus.owl#C14250)" .


###  http://purl.bioontology.org/ontology/STY/T002
<http://purl.bioontology.org/ontology/STY/T002> rdf:type owl:Class ;
                                                rdfs:subClassOf <http://purl.bioontology.org/ontology/STY/T204> ;
                                                rdfs:isDefinedBy "http://purl.bioontology.org/ontology/STY" ;
                                                rdfs:label "Plant"@en ;
                                                <http://www.w3.org/2004/02/skos/core#definition> "An organism having cellulose cell walls, growing by synthesis of inorganic substances, generally distinguished by the presence of chlorophyll, and lacking the power of locomotion. Plant parts are included here as well."@en .


###  http://purl.bioontology.org/ontology/STY/T004
<http://purl.bioontology.org/ontology/STY/T004> rdf:type owl:Class ;
                                                rdfs:subClassOf <http://purl.bioontology.org/ontology/STY/T204> ;
                                                rdfs:isDefinedBy "http://purl.bioontology.org/ontology/STY" ;
                                                rdfs:label "Fungus"@en ;
                                                <http://www.w3.org/2004/02/skos/core#definition> "A eukaryotic organism characterized by the absence of chlorophyll and the presence of a rigid cell wall. Included here are both slime molds and true fungi such as yeasts, molds, mildews, and mushrooms."@en .


###  http://purl.bioontology.org/ontology/STY/T005
<http://purl.bioontology.org/ontology/STY/T005> rdf:type owl:Class ;
                                                rdfs:subClassOf <http://purl.bioontology.org/ontology/STY/T001> ;
                                                rdfs:isDefinedBy "http://purl.bioontology.org/ontology/STY" ;
                                                rdfs:label "Virus"@en ;
                                                <http://www.w3.org/2004/02/skos/core#definition> "An organism consisting of a core of a single nucleic acid enclosed in a protective coat of protein. A virus may replicate only inside a host living cell. A virus exhibits some but not all of the usual characteristics of living things."@en .


###  http://purl.bioontology.org/ontology/STY/T007
<http://purl.bioontology.org/ontology/STY/T007> rdf:type owl:Class ;
                                                rdfs:subClassOf <http://purl.bioontology.org/ontology/STY/T001> ;
                                                rdfs:isDefinedBy "http://purl.bioontology.org/ontology/STY" ;
                                                rdfs:label "Bacterium"@en ;
                                                <http://www.w3.org/2004/02/skos/core#definition> "A small, typically one-celled, prokaryotic micro-organism."@en ;
                                                <http://www.w3.org/2004/02/skos/core#exactMatch> "Thesaurus:C14187 (http://ncicb.nci.nih.gov/xml/owl/EVS/Thesaurus.owl#C14187)" .


###  http://purl.bioontology.org/ontology/STY/T008
<http://purl.bioontology.org/ontology/STY/T008> rdf:type owl:Class ;
                                                rdfs:subClassOf <http://purl.bioontology.org/ontology/STY/T204> ;
                                                rdfs:isDefinedBy "http://purl.bioontology.org/ontology/STY" ;
                                                rdfs:label "Animal"@en ;
                                                <http://www.w3.org/2004/02/skos/core#definition> "An organism with eukaryotic cells, and lacking stiff cell walls, plastids and photosynthetic pigments."@en .


###  http://purl.bioontology.org/ontology/STY/T010
<http://purl.bioontology.org/ontology/STY/T010> rdf:type owl:Class ;
                                                rdfs:subClassOf <http://purl.bioontology.org/ontology/STY/T008> ;
                                                rdfs:isDefinedBy "http://purl.bioontology.org/ontology/STY" ;
                                                rdfs:label "Vertebrate"@en ;
                                                <http://www.w3.org/2004/02/skos/core#definition> "An animal which has a spinal column."@en .


###  http://purl.bioontology.org/ontology/STY/T011
<http://purl.bioontology.org/ontology/STY/T011> rdf:type owl:Class ;
                                                rdfs:subClassOf <http://purl.bioontology.org/ontology/STY/T010> ;
                                                rdfs:isDefinedBy "http://purl.bioontology.org/ontology/STY" ;
                                                rdfs:label "Amphibian"@en ;
                                                <http://www.w3.org/2004/02/skos/core#definition> "A cold-blooded, smooth-skinned vertebrate which characteristically hatches as an aquatic larva, breathing by gills. When mature, the amphibian breathes with lungs."@en .


###  http://purl.bioontology.org/ontology/STY/T012
<http://purl.bioontology.org/ontology/STY/T012> rdf:type owl:Class ;
                                                rdfs:subClassOf <http://purl.bioontology.org/ontology/STY/T010> ;
                                                rdfs:isDefinedBy "http://purl.bioontology.org/ontology/STY" ;
                                                rdfs:label "Bird"@en ;
                                                <http://www.w3.org/2004/02/skos/core#definition> "A vertebrate having a constant body temperature and characterized by the presence of feathers."@en .


###  http://purl.bioontology.org/ontology/STY/T013
<http://purl.bioontology.org/ontology/STY/T013> rdf:type owl:Class ;
                                                rdfs:subClassOf <http://purl.bioontology.org/ontology/STY/T010> ;
                                                rdfs:isDefinedBy "http://purl.bioontology.org/ontology/STY" ;
                                                rdfs:label "Fish"@en ;
                                                <http://www.w3.org/2004/02/skos/core#definition> "A cold-blooded aquatic vertebrate characterized by fins and breathing by gills. Included here are fishes having either a bony skeleton, such as a perch, or a cartilaginous skeleton, such as a shark, or those lacking a jaw, such as a lamprey or hagfish."@en .


###  http://purl.bioontology.org/ontology/STY/T014
<http://purl.bioontology.org/ontology/STY/T014> rdf:type owl:Class ;
                                                rdfs:subClassOf <http://purl.bioontology.org/ontology/STY/T010> ;
                                                rdfs:isDefinedBy "http://purl.bioontology.org/ontology/STY" ;
                                                rdfs:label "Reptile"@en ;
                                                <http://www.w3.org/2004/02/skos/core#definition> "A cold-blooded vertebrate having an external covering of scales or horny plates. Reptiles breathe by means of lungs and are generally egg-laying."@en .


###  http://purl.bioontology.org/ontology/STY/T015
<http://purl.bioontology.org/ontology/STY/T015> rdf:type owl:Class ;
                                                rdfs:subClassOf <http://purl.bioontology.org/ontology/STY/T010> ;
                                                rdfs:isDefinedBy "http://purl.bioontology.org/ontology/STY" ;
                                                rdfs:label "Mammal"@en ;
                                                <http://www.w3.org/2004/02/skos/core#definition> "A vertebrate having a constant body temperature and characterized by the presence of hair, mammary glands and sweat glands."@en .


###  http://purl.bioontology.org/ontology/STY/T051
<http://purl.bioontology.org/ontology/STY/T051> rdf:type owl:Class ;
                                                rdfs:subClassOf owl:Thing ;
                                                rdfs:isDefinedBy "http://purl.bioontology.org/ontology/STY" ;
                                                rdfs:label "Event"@en ;
                                                <http://www.w3.org/2004/02/skos/core#definition> "A broad type for grouping activities, processes and states."@en .


###  http://purl.bioontology.org/ontology/STY/T052
<http://purl.bioontology.org/ontology/STY/T052> rdf:type owl:Class ;
                                                rdfs:subClassOf <http://purl.bioontology.org/ontology/STY/T051> ;
                                                rdfs:isDefinedBy "http://purl.bioontology.org/ontology/STY" ;
                                                rdfs:label "Activity"@en ;
                                                <http://www.w3.org/2004/02/skos/core#definition> "An operation or series of operations that an organism or machine carries out or participates in."@en .


###  http://purl.bioontology.org/ontology/STY/T067
<http://purl.bioontology.org/ontology/STY/T067> rdf:type owl:Class ;
                                                rdfs:subClassOf <http://purl.bioontology.org/ontology/STY/T051> ;
                                                rdfs:isDefinedBy "http://purl.bioontology.org/ontology/STY" ;
                                                rdfs:label "Phenomenon or Process"@en ;
                                                <http://www.w3.org/2004/02/skos/core#definition> "A process or state which occurs naturally or as a result of an activity."@en .


###  http://purl.bioontology.org/ontology/STY/T071
<http://purl.bioontology.org/ontology/STY/T071> rdf:type owl:Class ;
                                                rdfs:subClassOf owl:Thing ;
                                                rdfs:isDefinedBy "http://purl.bioontology.org/ontology/STY" ;
                                                rdfs:label "Entity"@en ;
                                                <http://www.w3.org/2004/02/skos/core#definition> "A broad type for grouping physical and conceptual entities."@en .


###  http://purl.bioontology.org/ontology/STY/T072
<http://purl.bioontology.org/ontology/STY/T072> rdf:type owl:Class ;
                                                rdfs:subClassOf <http://purl.bioontology.org/ontology/STY/T071> ;
                                                rdfs:isDefinedBy "http://purl.bioontology.org/ontology/STY" ;
                                                rdfs:label "Physical Object"@en ;
                                                <http://www.w3.org/2004/02/skos/core#definition> "An object perceptible to the sense of vision or touch."@en .


###  http://purl.bioontology.org/ontology/STY/T077
<http://purl.bioontology.org/ontology/STY/T077> rdf:type owl:Class ;
                                                rdfs:subClassOf <http://purl.bioontology.org/ontology/STY/T071> ;
                                                rdfs:isDefinedBy "http://purl.bioontology.org/ontology/STY" ;
                                                rdfs:label "Conceptual Entity"@en ;
                                                <http://www.w3.org/2004/02/skos/core#definition> "A broad type for grouping abstract entities or concepts."@en ;
                                                <http://www.w3.org/2004/02/skos/core#exactMatch> "Thesaurus:C20181 (http://ncicb.nci.nih.gov/xml/owl/EVS/Thesaurus.owl#C20181)" .


###  http://purl.bioontology.org/ontology/STY/T170
<http://purl.bioontology.org/ontology/STY/T170> rdf:type owl:Class ;
                                                rdfs:subClassOf <http://purl.bioontology.org/ontology/STY/T077> ;
                                                rdfs:isDefinedBy "http://purl.bioontology.org/ontology/STY" ;
                                                rdfs:label "Intellectual Product"@en ;
                                                <http://www.w3.org/2004/02/skos/core#definition> "A conceptual entity resulting from human endeavor. Concepts assigned to this type generally refer to information created by humans for some purpose."@en .


###  http://purl.bioontology.org/ontology/STY/T194
<http://purl.bioontology.org/ontology/STY/T194> rdf:type owl:Class ;
                                                rdfs:subClassOf <http://purl.bioontology.org/ontology/STY/T001> ;
                                                rdfs:isDefinedBy "http://purl.bioontology.org/ontology/STY" ;
                                                rdfs:label "Archaeon"@en ;
                                                <http://www.w3.org/2004/02/skos/core#definition> "A member of one of the three domains of life, formerly called Archaebacteria under the taxon Bacteria, but now considered separate and distinct. Archaea are characterized by: 1) the presence of characteristic tRNAs and ribosomal RNAs; 2) the absence of peptidoglycan cell walls; 3) the presence of ether-linked lipids built from branched-chain subunits; and 4) their occurrence in unusual habitats. While archaea resemble bacteria in morphology and genomic organization, they resemble eukarya in their method of genomic replication."@en ;
                                                <http://www.w3.org/2004/02/skos/core#exactMatch> "Thesaurus:C61092 (http://ncicb.nci.nih.gov/xml/owl/EVS/Thesaurus.owl#C61092)" .


###  http://purl.bioontology.org/ontology/STY/T204
<http://purl.bioontology.org/ontology/STY/T204> rdf:type owl:Class ;
                                                rdfs:subClassOf <http://purl.bioontology.org/ontology/STY/T001> ;
                                                rdfs:isDefinedBy "http://purl.bioontology.org/ontology/STY" ;
                                                rdfs:label "Eukaryote"@en ;
                                                <http://www.w3.org/2004/02/skos/core#definition> "One of the three domains of life (the others being Bacteria and Archaea), also called Eukarya. These are organisms whose cells are enclosed in membranes and possess a nucleus. They comprise almost all multicellular and many unicellular organisms, and are traditionally divided into groups (sometimes called kingdoms) including Animals, Plants, Fungi, various Algae, and other taxa that were previously part of the old kingdom Protista."@en .


###  http://www.w3.org/2002/07/owl#Thing
owl:Thing rdf:type owl:Class .


###  https://purls.helmholtz-metadaten.de/ptroDKFZ000006
<https://purls.helmholtz-metadaten.de/ptroDKFZ000006> rdf:type owl:Class ;
                                                      rdfs:subClassOf <http://ncicb.nci.nih.gov/xml/owl/EVS/Thesaurus.owl#C25364> ;
                                                      <http://purl.org/dc/elements/1.1/creator> "Wahyu W. Hadiwikarta and Abumansur Sabyrrakhim" ;
                                                      rdfs:label "Animal Identifier" ;
                                                      <http://www.w3.org/2004/02/skos/core#definition> "An identifier which is used to uniquely identify an animal in a certain context (cohort, hospital, trial). Can be a pseudonym." .


###  https://purls.helmholtz-metadaten.de/ptroDKFZ000050
<https://purls.helmholtz-metadaten.de/ptroDKFZ000050> rdf:type owl:Class ;
                                                      rdfs:subClassOf <http://ncicb.nci.nih.gov/xml/owl/EVS/Thesaurus.owl#C25364> ;
                                                      owl:disjointWith <https://purls.helmholtz-metadaten.de/ptroDKFZ000059> ;
                                                      <http://purl.org/dc/elements/1.1/creator> "OGiraldo" ;
                                                      rdfs:comment "Term created to represent data in EX template that follows a long table structure." ;
                                                      rdfs:label "Treatment Session Identifier" ;
                                                      <http://www.w3.org/2004/02/skos/core#definition> "A sequence of characters used to identify a treatment session." .


###  https://purls.helmholtz-metadaten.de/ptroDKFZ000059
<https://purls.helmholtz-metadaten.de/ptroDKFZ000059> rdf:type owl:Class ;
                                                      rdfs:subClassOf <http://ncicb.nci.nih.gov/xml/owl/EVS/Thesaurus.owl#C25364> ;
                                                      <http://purl.org/dc/elements/1.1/creator> "OGiraldo" ;
                                                      rdfs:comment "Term created to represent data in LB template that follows a long table structure." ;
                                                      rdfs:label "Laboratory Record Identifier" ;
                                                      <http://www.w3.org/2004/02/skos/core#definition> "A sequence of characters used to identify laboratory records." .


###  https://purls.helmholtz-metadaten.de/ptroDKFZ000080
<https://purls.helmholtz-metadaten.de/ptroDKFZ000080> rdf:type owl:Class ;
                                                      rdfs:subClassOf <http://ncicb.nci.nih.gov/xml/owl/EVS/Thesaurus.owl#C25364> ;
                                                      <http://purl.org/dc/elements/1.1/creator> "OGiraldo" ;
                                                      rdfs:comment "Term created to represent data in BW template that follows a long table structure." ;
                                                      rdfs:label "Body Weight Identifier" ;
                                                      <http://www.w3.org/2004/02/skos/core#definition> "A sequence of characters used to identify body weight records." .


###  https://purls.helmholtz-metadaten.de/ptroDKFZ000087
<https://purls.helmholtz-metadaten.de/ptroDKFZ000087> rdf:type owl:Class ;
                                                      rdfs:subClassOf <http://ncicb.nci.nih.gov/xml/owl/EVS/Thesaurus.owl#C25364> ;
                                                      <http://purl.org/dc/elements/1.1/creator> "OGiraldo" ;
                                                      rdfs:comment "Term created to represent data in PR template that follows a long table structure." ;
                                                      rdfs:label "Procedure Identifier" ;
                                                      <http://www.w3.org/2004/02/skos/core#definition> "A sequence of characters used to identify procedure records." .


###  Generated by the OWL API (version 5.1.18) https://github.com/owlcs/owlapi/
